Filled the gap between the Coverage invariant and the last two serializability conditions.

src/RqRsInvAtomic.v
@@ -10,18 +10,22 @@ Set Implicit Arguments.
 Open Scope list.
 Open Scope fmap.
 
-Fixpoint UniqueIn {A} (a: A) (l: list A) :=
-  match l with
-  | nil => False
-  | b :: m => (b = a /\ ~ In a m) \/ (b <> a /\ UniqueIn a m)
-  end.
+(* Fixpoint UniqueIn {A} (a: A) (l: list A) := *)
+(*   match l with *)
+(*   | nil => False *)
+(*   | b :: m => (b = a /\ ~ In a m) \/ (b <> a /\ UniqueIn a m) *)
+(*   end. *)
 
-Section MsgOutCases.
+Section Coverage.
   Context {oifc: OStateIfc}.
   Variables (dtr: DTree)
             (sys: System oifc).
   Hypothesis (Hrrs: RqRsSys dtr sys).
 
+  Definition RqUpMsgFrom (oidx: IdxT) (idm: Id Msg) :=
+    msg_type (valOf idm) = MRq /\
+    rqEdgeUpFrom dtr oidx = Some (idOf idm).
+  
   Definition RsDownMsgTo (oidx: IdxT) (idm: Id Msg) :=
     msg_type (valOf idm) = MRs /\
     edgeDownTo dtr oidx = Some (idOf idm).
@@ -36,165 +40,321 @@ Section MsgOutCases.
 
   Ltac disc_msg_case :=
     match goal with
+    | [H: RqUpMsgFrom _ _ |- _] => destruct H
     | [H: RsDownMsgTo _ _ |- _] => destruct H
     | [H: RqDownMsgTo _ _ |- _] => destruct H
     | [H: RsUpMsgFrom _ _ |- _] => destruct H
     end.
 
-  Definition NoDownLock (oidx: IdxT) (orqs: ORqs Msg) :=
-    orqs@[oidx] >>=[True] (fun orq => orq@[downRq] = None).
+  Section OnAtomic.
 
-  Definition NoDownLocks (oinds: list IdxT) (orqs: ORqs Msg) :=
-    forall oidx,
-      In oidx oinds -> NoDownLock oidx orqs.
+    Variables (oinds: list IdxT) (orqs1 orqs2: ORqs Msg).
 
-  Definition NoDownLocks2 (oinds1: list IdxT) (oinds2: list IdxT) (orqs: ORqs Msg) :=
-    forall oidx,
-      In oidx oinds1 ->
-      In oidx oinds2 ->
-      NoDownLock oidx orqs.
+    Definition NoDownLock (oidx: IdxT) :=
+      orqs2@[oidx] >>=[True] (fun orq => orq@[downRq] = None).
 
-  Definition IndsDisjTree (ridx: IdxT) (oinds: list IdxT) :=
-    DisjList oinds (subtreeIndsOf dtr ridx).
+    Definition NoDownLocks := 
+      forall oidx, In oidx oinds -> NoDownLock oidx.
 
-  Definition RsDownMsgOutInv (oidx: IdxT) (rsDown: Id Msg) (oinds: list IdxT) :=
-    RsDownMsgTo oidx rsDown /\
-    IndsDisjTree oidx oinds.
+    Definition NoDownLocks2 (oinds2: list IdxT) :=
+      forall oidx,
+        In oidx oinds ->
+        In oidx oinds2 ->
+        NoDownLock oidx.
 
-  Definition RqDownMsgOutInv (oidx: IdxT) (rqDown: Id Msg) (oinds: list IdxT) :=
-    RqDownMsgTo oidx rqDown /\
-    IndsDisjTree oidx oinds.
+    Definition IndsInTree (ridx: IdxT) :=
+      SubList oinds (subtreeIndsOf dtr ridx).
+    
+    Definition IndsDisjTree (ridx: IdxT) :=
+      DisjList oinds (subtreeIndsOf dtr ridx).
 
-  Definition RsUpMsgOutInv (oidx: IdxT) (rsUp: Id Msg) (orqs: ORqs Msg) (oinds: list IdxT) :=
-    RsUpMsgFrom oidx rsUp /\
-    NoDownLocks2 oinds (subtreeIndsOf dtr oidx) orqs.
+    Definition UpLocked (oidx: IdxT) (rqiu: RqInfo Msg) :=
+      orqs2@[oidx] >>=[False]
+           (fun orq2 => orq2@[upRq] = Some rqiu).
+    
+    Definition UpLockedNew (oidx: IdxT) (rqiu: RqInfo Msg) :=
+      orqs2@[oidx] >>=[False]
+           (fun orq2 =>
+              orq2@[upRq] = Some rqiu /\
+              orqs1@[oidx] >>=[True] (fun orq1 => orq1@[upRq] = None)).
 
-  Definition DownLockCoverInv (oidx: IdxT) (rqid: RqInfo Msg) (oinds: list IdxT) :=
-    forall cidx rsUp,
-      parentIdxOf dtr cidx = Some oidx ->
-      rsEdgeUpFrom dtr cidx = Some rsUp ->
-      ~ In rsUp rqid.(rqi_minds_rss) ->
-      IndsDisjTree cidx oinds.
+    Definition DownLocked (oidx: IdxT) (rqid: RqInfo Msg) :=
+      orqs2@[oidx] >>=[False]
+           (fun orq2 => orq2@[downRq] = Some rqid).
 
-  Definition DownLocksCoverInv (orqs: ORqs Msg) (oinds: list IdxT) :=
-    forall oidx orq rqid,
-      In oidx oinds ->
-      orqs@[oidx] = Some orq ->
-      orq@[downRq] = Some rqid ->
-      DownLockCoverInv oidx rqid oinds.
+    Definition DisjExceptUpLocked (tidx: IdxT) :=
+      forall oidx,
+        In oidx oinds ->
+        forall rqiu,
+          ~ UpLockedNew oidx rqiu ->
+          ~ In oidx (subtreeIndsOf dtr tidx).
 
-  Definition DownLockInRoot (roidx: IdxT) (orqs: ORqs Msg) (oinds: list IdxT) :=
-    forall sidx sorq srqid,
-      In sidx oinds ->
-      orqs@[sidx] = Some sorq ->
-      sorq@[downRq] = Some srqid ->
-      In sidx (subtreeIndsOf dtr roidx).
-  
-  Definition DownLockRootInv (orqs: ORqs Msg) (oinds: list IdxT) :=
-    forall roidx rorq rrqid rcidx rrsUp,
-      In roidx oinds ->
-      orqs@[roidx] = Some rorq ->
-      rorq@[downRq] = Some rrqid ->
-      parentIdxOf dtr rcidx = Some roidx ->
-      edgeDownTo dtr rcidx = Some (rrqid.(rqi_midx_rsb)) ->
-      rsEdgeUpFrom dtr rcidx = Some rrsUp ->
-      ~ In rrsUp rrqid.(rqi_minds_rss) /\
-      IndsDisjTree rcidx oinds /\
-      DownLockInRoot roidx orqs oinds.
+    Definition RqUpMsgOutInv (oidx: IdxT) (rqUp: Id Msg) :=
+      RqUpMsgFrom oidx rqUp.
 
-  Definition DownLockNorm (orq: ORq Msg): nat :=
-    orq@[downRq] >>=[0] (fun rqid => List.length rqid.(rqi_minds_rss) - 1).
+    Definition RsDownMsgOutInv (oidx: IdxT) (rsDown: Id Msg) :=
+      RsDownMsgTo oidx rsDown /\ DisjExceptUpLocked oidx.
 
-  Fixpoint DownLocksNorm (oinds: list IdxT) (orqs: ORqs Msg): nat :=
-    match oinds with
-    | nil => 0
-    | hoind :: toinds =>
-      (orqs@[hoind] >>=[0] (fun orq => DownLockNorm orq)) +
-      DownLocksNorm toinds orqs
-    end.
+    Definition RqDownMsgOutInv (oidx: IdxT) (rqDown: Id Msg) :=
+      RqDownMsgTo oidx rqDown /\ IndsDisjTree oidx.
 
-  Definition MsgOutsNormInv (orqs: ORqs Msg) (oinds: list IdxT) (eouts: list (Id Msg)) :=
-    List.length (idsOf eouts) = DownLocksNorm oinds orqs + 1.
-  
-  Inductive MsgOutsCases (orqs: ORqs Msg) (oinds: list IdxT): list (Id Msg) -> Prop :=
-  | MsgOutsRsDown: (* Only one live RsDown message *)
-      forall oidx rsDown,
-        RsDownMsgOutInv oidx rsDown oinds ->
-        NoDownLocks oinds orqs ->
-        MsgOutsCases orqs oinds [rsDown]
-  | MsgOutsRqDownRsUp: (* RqDown or RsUp messages *)
-      forall eouts,
-        NoDup (idsOf eouts) ->
-        Forall (fun eout =>
-                  exists oidx,
-                    RqDownMsgOutInv oidx eout oinds \/
-                    RsUpMsgOutInv oidx eout orqs oinds) eouts ->
-        DownLocksCoverInv orqs oinds ->
-        DownLockRootInv orqs oinds ->
-        MsgOutsNormInv orqs oinds eouts ->
+    Definition RsUpMsgOutInv (oidx: IdxT) (rsUp: Id Msg) :=
+      RsUpMsgFrom oidx rsUp /\ NoDownLocks2 (subtreeIndsOf dtr oidx).
 
-        (** Currently I don't think we explicitly need to state all RqDown/RsUp
-         * subtrees are disjoint to each other -- we can prove this using 
-         * their respective invariants and the Up/DownLock invariants (already
-         * proven in [RqRsInvLock.v]).
-         *)
-        MsgOutsCases orqs oinds eouts.
+    Definition UpLockCoverInv (oidx: IdxT) (rqiu: RqInfo Msg) :=
+      forall cidx down,
+        parentIdxOf dtr cidx = Some oidx ->
+        edgeDownTo dtr cidx = Some down ->
+        down <> rqiu.(rqi_midx_rsb) ->
+        IndsDisjTree cidx.
+
+    Definition UpLocksCoverInv :=
+      forall oidx rqiu,
+        In oidx oinds ->
+        UpLocked oidx rqiu ->
+        UpLockCoverInv oidx rqiu.
+
+    Definition DownLockCoverInv (oidx: IdxT) (rqid: RqInfo Msg) :=
+      forall cidx rsUp,
+        parentIdxOf dtr cidx = Some oidx ->
+        rsEdgeUpFrom dtr cidx = Some rsUp ->
+        ~ In rsUp rqid.(rqi_minds_rss) ->
+        IndsDisjTree cidx.
+
+    Definition DownLocksCoverInv :=
+      forall oidx rqid,
+        In oidx oinds ->
+        DownLocked oidx rqid ->
+        DownLockCoverInv oidx rqid.
+
+    (* The root of downlocks is the one that also has a downlock but
+     * the return index ([rqi_midx_rsb]) is one of children.
+     *)
+    Definition DownLockRoot
+               (roidx: IdxT) (rorq: ORq Msg)
+               (rrqid: RqInfo Msg) (rcidx: IdxT) :=
+      In roidx oinds /\
+      DownLocked roidx rrqid /\
+      parentIdxOf dtr rcidx = Some roidx /\
+      edgeDownTo dtr rcidx = Some (rrqid.(rqi_midx_rsb)).
+
+    Definition NoDownLockRoot :=
+      forall roidx rorq rrqid rcidx,
+        In roidx oinds -> ~ DownLockRoot roidx rorq rrqid rcidx.
+
+    Definition DownLockInRoot (roidx: IdxT) :=
+      forall sidx srqid,
+        In sidx oinds ->
+        DownLocked sidx srqid ->
+        In sidx (subtreeIndsOf dtr roidx).
+    
+    Definition DownLockRootInv (roidx: IdxT) (rcidx: IdxT) :=
+      DownLockInRoot roidx /\ DisjExceptUpLocked rcidx.
+
+    Definition DownLockNorm (oidx: IdxT): nat :=
+      orqs2@[oidx] >>=[0]
+           (fun orq =>
+              orq@[downRq] >>=[0]
+                 (fun rqid => List.length rqid.(rqi_minds_rss) - 1)).
+
+    Fixpoint DownLocksNorm (doinds: list IdxT): nat :=
+      match doinds with
+      | nil => 0
+      | hoind :: toinds =>
+        DownLockNorm hoind + DownLocksNorm toinds
+      end.
+
+    Definition MsgOutsNormInv (roidx: IdxT) (eouts: list (Id Msg)) :=
+      List.length (idsOf eouts) =
+      DownLockNorm roidx +
+      DownLocksNorm (remove eq_nat_dec roidx oinds) + 1.
+
+    Inductive MsgOutsCases: list (Id Msg) -> Prop :=
+    | MsgOutsRqUp: (* Only one live RqUp message *)
+        forall oidx rqUp,
+          RqUpMsgOutInv oidx rqUp ->
+          UpLocksCoverInv ->
+          MsgOutsCases [rqUp]
+    | MsgOutsRsDown: (* Only one live RsDown message *)
+        forall oidx rsDown,
+          RsDownMsgOutInv oidx rsDown ->
+          NoDownLocks ->
+          MsgOutsCases [rsDown]
+    | MsgOutsRqDownRsUp: (* RqDown or RsUp messages *)
+        forall eouts,
+          NoDup (idsOf eouts) ->
+          Forall (fun eout =>
+                    exists oidx,
+                      RqDownMsgOutInv oidx eout \/
+                      RsUpMsgOutInv oidx eout) eouts ->
+          DownLocksCoverInv ->
+          (forall roidx rorq rrqid rcidx,
+              DownLockRoot roidx rorq rrqid rcidx ->
+              DownLockRootInv roidx rcidx /\
+              MsgOutsNormInv roidx eouts) ->
+          MsgOutsCases eouts.
+
+  End OnAtomic.
+
+  (*! Facts *)
 
   Ltac disc_rule_custom ::=
     try disc_footprints_ok;
     try disc_messages_in;
     try disc_msg_case.
 
-  Ltac solve_msg_out_cases_step :=
-    match goal with
-    | [H: edgeDownTo _ _ = Some ?midx
-       |- RqDownMsgOutInv _ (?midx, _) _ \/
-          RsUpMsgOutInv _ (?midx, _) _ _] => left
-    | [H: rsEdgeUpFrom _ _ = Some ?midx
-       |- RqDownMsgOutInv _ (?midx, _) _ \/
-          RsUpMsgOutInv _ (?midx, _) _ _] => right
-    | [ |- RsDownMsgOutInv _ _ _] => split
-    | [ |- RqDownMsgOutInv _ _ _] => split
-    | [ |- RsUpMsgOutInv _ _ _ _] => split
-                                       
-    | [ |- DownLocksCoverInv _ _] => red; intros
-    | [ |- DownLockCoverInv _ _ _] => red; intros
-    | [ |- DownLockRootInv _ _] => red; intros; repeat ssplit
-    | [ |- DownLockInRoot _ _ _] => red; intros
+  Lemma disjExceptUpLocked_no_UpLockedNew_disj:
+    forall oinds orqs1 orqs2 tidx,
+      DisjExceptUpLocked oinds orqs1 orqs2 tidx ->
+      Forall (fun oidx =>
+                forall rqiu,
+                  ~ UpLockedNew orqs1 orqs2 oidx rqiu) oinds ->
+      DisjList oinds (subtreeIndsOf dtr tidx).
+  Proof.
+    unfold DisjExceptUpLocked; intros.
+    apply (DisjList_false_spec eq_nat_dec).
+    intros oidx ? ?.
+    rewrite Forall_forall in H0.
+    specialize (H0 _ H1).
+    specialize (H _ H1).
+    eapply H
+      with (rqiu:= {| rqi_msg := {| msg_id := 0;
+                                    msg_type := false;
+                                    msg_value := VUnit |};
+                      rqi_minds_rss := nil;
+                      rqi_midx_rsb := 0 |}); eauto.
+  Qed.
+  
+  Lemma step_NonRqUp_no_new_uplocks:
+    forall st1 oidx ridx rins routs st2,
+      Reachable (steps step_m) sys st1 ->
+      step_m sys st1 (RlblInt oidx ridx rins routs) st2 ->
+      NonRqUpL dtr (RlblInt oidx ridx rins routs) ->
+      forall rqiu,
+        ~ UpLockedNew st1.(bst_orqs) st2.(bst_orqs) oidx rqiu.
+  Proof.
+    destruct Hrrs as [? [? ?]]; intros.
+    pose proof (footprints_ok H0 H2).
+    inv_step.
+    good_rqrs_rule_get rule.
+    good_rqrs_rule_cases rule; simpl in *.
 
-    | [ |- MsgOutsNormInv _ _ _] => red; simpl
+    - disc_rule_conds.
+      intro Hx; red in Hx; repeat (simpl in Hx; mred).
+      dest; congruence.
 
-    | [ |- RqDownMsgTo _ _] => red; eauto; fail
-    | [ |- RsDownMsgTo _ _] => red; eauto; fail
-    | [ |- RsUpMsgFrom _ _] => red; eauto; fail
+    - disc_rule_conds.
+      intro Hx; red in Hx; repeat (simpl in Hx; mred).
+      dest; congruence.
 
-    | [ |- IndsDisjTree _ _] => red; simpl
-    | [ |- NoDownLocks _ _] => simpl; red; intros
-    | [ |- NoDownLock _ _] => red; repeat (mred; simpl); fail
-    | [ |- NoDownLocks2 _ _ _] => simpl; red; intros
+    - disc_rule_conds.
+      + pose proof (rqEdgeUpFrom_Some H _ H7).
+        destruct H15 as [rsUp [down [pidx ?]]]; dest.
+        elim (H4 pidx).
+        red; do 2 eexists; eauto.
+      + intro Hx; red in Hx; repeat (simpl in Hx; mred).
+        dest; congruence.
+      + intro Hx; red in Hx; repeat (simpl in Hx; mred).
+        dest; congruence.
 
-    | [H: In _ [_] |- _] => Common.dest_in
-    | [H: In _ (oindsOf [_]) |- _] => Common.dest_in
-    | [ |- DisjList [_] _] => apply (DisjList_singleton_1 eq_nat_dec)
-    | [H: parentIdxOf _ ?cidx = Some ?pidx
-       |- ~ In ?pidx (subtreeIndsOf _ ?cidx)] =>
-      apply parent_not_in_subtree; assumption
-    | [ |- Forall _ _] => repeat constructor
-    | [ |- NoDup _] => clear; simpl; repeat constructor; firstorder; fail
-    | [ |- exists _, _] => eexists
-    | [ |- context [(Some _) >>=[_] (fun _ => _)]] => simpl
-    end.
+    - good_footprint_get (obj_idx obj).
+      disc_rule_conds.
+      + intro Hx; red in Hx; repeat (simpl in Hx; mred).
+        dest; congruence.
+      + intro Hx; red in Hx; repeat (simpl in Hx; mred).
+        dest; congruence.
+      + intro Hx; red in Hx; repeat (simpl in Hx; mred).
+        dest; congruence.
 
-  Ltac solve_msg_out_cases :=
-    repeat (try solve_msg_out_cases_step; mred).
+    - disc_rule_conds.
+      intro Hx; red in Hx; repeat (simpl in Hx; mred).
+      dest; congruence.
+  Qed.
 
-  Ltac solve_msg_out_cases_bt :=
-    try (solve_msg_out_cases; fail).
+  Lemma upLockedNew_not_trans:
+    forall orqs1 orqs2 orqs3 oidx,
+      (forall rqiu, ~ UpLockedNew orqs1 orqs2 oidx rqiu) ->
+      (forall rqiu, ~ UpLockedNew orqs2 orqs3 oidx rqiu) ->
+      forall rqiu,
+        ~ UpLockedNew orqs1 orqs3 oidx rqiu.
+  Proof.
+    unfold UpLockedNew; intros; intro Hx.
+    destruct (orqs3@[oidx]) as [orq3|]; simpl in *; dest; auto.
+    rewrite H1 in *; clear H1.
+    destruct (orqs2@[oidx]) as [orq2|]; simpl in *; dest.
+    - destruct (orq2@[upRq]) as [rqiu2|]; simpl in *.
+      + elim (H rqiu2); auto.
+      + elim (H0 rqiu); auto.
+    - elim (H0 rqiu); auto.
+  Qed.
 
+  Lemma upLockedNew_index_eq_1:
+    forall orqs orqs1 orqs2 oidx rqiu,
+      orqs1@[oidx] = orqs2@[oidx] ->
+      (UpLockedNew orqs orqs1 oidx rqiu <->
+       UpLockedNew orqs orqs2 oidx rqiu).
+  Proof.
+    unfold UpLockedNew; intros.
+    rewrite H; intuition idtac.
+  Qed.
+
+  Lemma upLockedNew_index_eq_2:
+    forall orqs orqs1 orqs2 oidx rqiu,
+      orqs1@[oidx] = orqs2@[oidx] ->
+      (UpLockedNew orqs1 orqs oidx rqiu <->
+       UpLockedNew orqs2 orqs oidx rqiu).
+  Proof.
+    unfold UpLockedNew; intros.
+    rewrite H; intuition idtac.
+  Qed.
+
+  Lemma atomic_NonRqUp_no_new_uplocks:
+    forall inits ins hst outs eouts,
+      Atomic msg_dec inits ins hst outs eouts ->
+      Forall (NonRqUpL dtr) hst ->
+      forall s1 s2,
+        Reachable (steps step_m) sys s1 ->
+        steps step_m sys s1 hst s2 ->
+        Forall (fun oidx =>
+                  forall rqiu,
+                    ~ UpLockedNew s1.(bst_orqs) s2.(bst_orqs) oidx rqiu) (oindsOf hst).
+  Proof.
+    destruct Hrrs as [? [? ?]].
+    induction 1; simpl; intros; subst.
+    - inv_steps; inv H2; clear H7.
+      repeat constructor.
+      eapply step_NonRqUp_no_new_uplocks; eauto.
+    - inv_steps; inv H8.
+      specialize (IHAtomic H10 _ _ H9 H11).
+      constructor.
+      + destruct (in_dec eq_nat_dec oidx (oindsOf hst)).
+        * intros; intro Hx.
+          rewrite Forall_forall in IHAtomic.
+          specialize (IHAtomic _ i).
+          eapply upLockedNew_not_trans; eauto.
+          eapply step_NonRqUp_no_new_uplocks; eauto.
+        * pose proof H11.
+          eapply steps_locks_unaffected in H5; [|eassumption].
+          intros; intro Hx.
+          rewrite upLockedNew_index_eq_2 in Hx; [|eassumption].
+          eapply step_NonRqUp_no_new_uplocks with (st1:= st2); eauto.
+      + apply Forall_forall; intros uidx ?.
+        rewrite Forall_forall in IHAtomic; specialize (IHAtomic _ H5).
+        destruct (eq_nat_dec uidx oidx); subst.
+        * eapply upLockedNew_not_trans; eauto.
+          eapply step_NonRqUp_no_new_uplocks; eauto.
+        * intros; intro Hx.
+          elim (IHAtomic rqiu).
+          rewrite upLockedNew_index_eq_1; [eassumption|].
+          eapply steps_locks_unaffected.
+          { eapply steps_singleton; eassumption. }
+          { simpl; intros; intuition auto. }
+  Qed.
+  
   Lemma noDownLock_orqs_downRq_remove:
     forall oidx orqs ridx rorq,
-      NoDownLock oidx orqs ->
-      NoDownLock oidx (orqs +[ridx <- rorq -[downRq]]).
+      NoDownLock orqs oidx ->
+      NoDownLock (orqs +[ridx <- rorq -[downRq]]) oidx.
   Proof.
     unfold NoDownLock; intros.
     destruct (eq_nat_dec ridx oidx); subst; repeat (simpl; mred).
@@ -202,8 +362,8 @@ Section MsgOutCases.
 
   Lemma noDownLocks2_orqs_downRq_remove:
     forall oinds tinds orqs ridx rorq,
-      NoDownLocks2 oinds tinds orqs ->
-      NoDownLocks2 oinds tinds (orqs +[ridx <- rorq -[downRq]]).
+      NoDownLocks2 oinds orqs tinds ->
+      NoDownLocks2 oinds (orqs +[ridx <- rorq -[downRq]]) tinds.
   Proof.
     unfold NoDownLocks2; intros.
     eapply noDownLock_orqs_downRq_remove; auto.
@@ -211,36 +371,38 @@ Section MsgOutCases.
 
   Lemma downLockInRoot_orqs_downRq_remove:
     forall oidx orqs oinds ridx rorq,
-      DownLockInRoot oidx orqs oinds ->
-      DownLockInRoot oidx (orqs +[ridx <- rorq -[downRq]]) oinds.
+      DownLockInRoot oinds orqs oidx ->
+      DownLockInRoot oinds (orqs +[ridx <- rorq -[downRq]]) oidx.
   Proof.
     unfold DownLockInRoot; intros.
-    eapply H; eauto.
-    destruct (eq_nat_dec sidx ridx); subst; mred.
+    eapply H with (srqid:= srqid); eauto.
+    unfold DownLocked in *.
+    destruct (eq_nat_dec sidx ridx);
+      subst; repeat (simpl in *; mred).
   Qed.
 
   Lemma rsUpMsgOutInv_orqs_downRq_remove:
     forall oidx rsUp orqs oinds ridx rorq,
-      RsUpMsgOutInv oidx rsUp orqs oinds ->
-      RsUpMsgOutInv oidx rsUp (orqs +[ridx <- rorq -[downRq]]) oinds.
+      RsUpMsgOutInv oinds orqs oidx rsUp ->
+      RsUpMsgOutInv oinds (orqs +[ridx <- rorq -[downRq]]) oidx rsUp.
   Proof.
     intros; destruct H.
     split; [assumption|].
     apply noDownLocks2_orqs_downRq_remove; auto.
   Qed.
-      
+  
   Lemma noDownLocks2_oinds_tl:
     forall oinds oidx tinds orqs,
-      NoDownLocks2 (oidx :: oinds) tinds orqs ->
-      NoDownLocks2 oinds tinds orqs.
+      NoDownLocks2 (oidx :: oinds) orqs tinds ->
+      NoDownLocks2 oinds orqs tinds.
   Proof.
     unfold NoDownLocks2; intros; firstorder.
   Qed.
 
   Lemma rsUpMsgOutInv_oinds_tl:
     forall ridx rsUp orqs oinds oidx,
-      RsUpMsgOutInv ridx rsUp orqs (oidx :: oinds) ->
-      RsUpMsgOutInv ridx rsUp orqs oinds.
+      RsUpMsgOutInv (oidx :: oinds) orqs ridx rsUp ->
+      RsUpMsgOutInv oinds orqs ridx rsUp.
   Proof.
     unfold RsUpMsgOutInv; intros; dest.
     split; auto.
@@ -249,8 +411,8 @@ Section MsgOutCases.
 
   Lemma downLockCoverInv_oinds_tl:
     forall ridx rqi oinds oidx,
-      DownLockCoverInv ridx rqi (oidx :: oinds) ->
-      DownLockCoverInv ridx rqi oinds.
+      DownLockCoverInv (oidx :: oinds) ridx rqi ->
+      DownLockCoverInv oinds ridx rqi.
   Proof.
     unfold DownLockCoverInv; intros.
     specialize (H _ _ H0 H1 H2).
@@ -259,8 +421,8 @@ Section MsgOutCases.
 
   Lemma downLockInRoot_oinds_tl:
     forall ridx orqs oinds oidx,
-      DownLockInRoot ridx orqs (oidx :: oinds) ->
-      DownLockInRoot ridx orqs oinds.
+      DownLockInRoot (oidx :: oinds) ridx orqs ->
+      DownLockInRoot oinds ridx orqs.
   Proof.
     unfold DownLockInRoot; intros.
     eapply H; eauto.
@@ -270,11 +432,11 @@ Section MsgOutCases.
   Lemma downLocksNorm_orqs_add:
     forall oinds orqs ooidx orq,
       ~ In ooidx oinds ->
-      DownLocksNorm oinds (orqs +[ooidx <- orq]) =
-      DownLocksNorm oinds orqs.
+      DownLocksNorm (orqs +[ooidx <- orq]) oinds =
+      DownLocksNorm orqs oinds.
   Proof.
     induction oinds as [|oidx oinds]; simpl; intros; [reflexivity|].
-    mred.
+    unfold DownLockNorm; mred.
     destruct (in_dec eq_nat_dec ooidx oinds); [exfalso; auto|].
     rewrite IHoinds by assumption.
     reflexivity.
@@ -283,7 +445,7 @@ Section MsgOutCases.
   Lemma downLocksNorm_NoDownLocks_zero:
     forall oinds orqs,
       NoDownLocks oinds orqs ->
-      DownLocksNorm oinds orqs = 0.
+      DownLocksNorm orqs oinds = 0.
   Proof.
     induction oinds as [|oidx oinds]; simpl; intros; [reflexivity|].
     pose proof (H _ (or_introl eq_refl)).
@@ -292,6 +454,7 @@ Section MsgOutCases.
       eapply H; right; assumption.
     }
     red in H0.
+    unfold DownLockNorm.
     destruct (orqs@[oidx]); simpl in *; auto.
     unfold DownLockNorm; rewrite H0; simpl; auto.
   Qed.
@@ -301,18 +464,21 @@ Section MsgOutCases.
       oidx <> ridx ->
       In oidx oinds ->
       rqi_minds_rss rqi = idsOf rsUps ->
-      (forall rsUp, In rsUp rsUps -> exists cidx, RsUpMsgOutInv cidx rsUp orqs oinds) ->
-      DownLockCoverInv ridx rqi oinds ->
-      DownLockInRoot ridx orqs oinds ->
-      NoDownLock oidx orqs.
+      (forall rsUp,
+          In rsUp rsUps ->
+          exists cidx, RsUpMsgOutInv oinds orqs cidx rsUp) ->
+      DownLockCoverInv oinds ridx rqi ->
+      DownLockInRoot oinds orqs ridx ->
+      NoDownLock orqs oidx.
   Proof.
     destruct Hrrs as [? [? ?]]; intros; red.
-    remember (orqs@[oidx]) as orq; destruct orq as [orq|]; [|reflexivity].
-    apply eq_sym in Heqorq; simpl.
-    remember (orq@[downRq]) as rqid; destruct rqid as [rqid|]; [|reflexivity].
-    apply eq_sym in Heqrqid.
+    destruct (orqs@[oidx]) as [orq|] eqn:Horq; [|reflexivity].
+    simpl; destruct (orq@[downRq]) as [rqid|] eqn:Hrqid; [|reflexivity].
     exfalso.
-    specialize (H7 _ _ _ H3 Heqorq Heqrqid).
+    specialize (H7 oidx rqid H3).
+    unfold DownLocked in H7.
+    rewrite Horq in H7; simpl in H7.
+    specialize (H7 Hrqid).
     apply subtreeIndsOf_composed in H7; [|apply Hrrs].
     destruct H7; [subst; intuition|].
     destruct H7 as [cidx [? ?]].
@@ -336,9 +502,11 @@ Section MsgOutCases.
       orqs@[ridx] = Some rorq ->
       rorq@[downRq] = Some rqi ->
       rqi.(rqi_minds_rss) = idsOf rsUps ->
-      (forall rsUp, In rsUp rsUps -> exists cidx, RsUpMsgOutInv cidx rsUp orqs oinds) ->
-      DownLockCoverInv ridx rqi oinds ->
-      DownLockInRoot ridx orqs oinds ->
+      (forall rsUp,
+          In rsUp rsUps ->
+          exists cidx, RsUpMsgOutInv oinds orqs cidx rsUp) ->
+      DownLockCoverInv oinds ridx rqi ->
+      DownLockInRoot oinds orqs ridx ->
       NoDownLocks oinds orqs.
   Proof.
     destruct Hrrs as [? [? ?]]; intros.
@@ -361,59 +529,60 @@ Section MsgOutCases.
       + assumption.
   Qed.
   
-  Lemma downLocksNorm_rsUps:
-    forall orqs oinds ridx (rorq: ORq Msg) rqi rsUps,
-      UniqueIn ridx oinds ->
-      orqs@[ridx] = Some rorq ->
-      rorq@[downRq] = Some rqi ->
-      rsUps <> nil ->
-      rqi.(rqi_minds_rss) = idsOf rsUps ->
-      (forall rsUp, In rsUp rsUps -> exists cidx, RsUpMsgOutInv cidx rsUp orqs oinds) ->
-      DownLockCoverInv ridx rqi oinds ->
-      DownLockInRoot ridx orqs oinds ->
-      DownLocksNorm oinds orqs = length (idsOf rsUps) - 1.
-  Proof.
-    destruct Hrrs as [? [? ?]]; intros.
-    assert (length (idsOf rsUps) > 0)
-      by (destruct rsUps; [exfalso; auto|simpl; omega]).
-    clear H5.
+  (* Lemma downLocksNorm_rsUps: *)
+  (*   forall orqs oinds ridx (rorq: ORq Msg) rqi rsUps, *)
+  (*     orqs@[ridx] = Some rorq -> *)
+  (*     rorq@[downRq] = Some rqi -> *)
+  (*     rsUps <> nil -> *)
+  (*     rqi.(rqi_minds_rss) = idsOf rsUps -> *)
+  (*     (forall rsUp, *)
+  (*         In rsUp rsUps -> exists cidx, RsUpMsgOutInv cidx rsUp orqs oinds) -> *)
+  (*     DownLockCoverInv ridx rqi oinds -> *)
+  (*     DownLockInRoot ridx orqs oinds -> *)
+  (*     DownLocksNorm oinds orqs = length (idsOf rsUps) - 1. *)
+  (* Proof. *)
+  (*   destruct Hrrs as [? [? ?]]; intros. *)
+  (*   assert (length (idsOf rsUps) > 0) *)
+  (*     by (destruct rsUps; [exfalso; auto|simpl; omega]). *)
+  (*   clear H5. *)
 
-    induction oinds as [|oidx oinds]; simpl; intros; [exfalso; auto|].
-    destruct H2; dest.
-    - clear IHoinds.
-      subst; mred; simpl.
-      unfold DownLockNorm; repeat (simpl; mred).
-      rewrite H6.
-      rewrite downLocksNorm_NoDownLocks_zero; [omega|].
-      eapply downLocksNorm_rsUps_NoDownLocks; eauto.
-      + intros.
-        specialize (H7 _ H2); destruct H7 as [cidx ?].
-        eexists; eapply rsUpMsgOutInv_oinds_tl; eassumption.
-      + eapply downLockCoverInv_oinds_tl; eassumption.
-      + eapply downLockInRoot_oinds_tl; eassumption.
-    - replace ((orqs@[oidx]) >>=[0] (fun orq => DownLockNorm orq)) with 0.
-      + simpl; eapply IHoinds.
-        * assumption.
-        * intros.
-          specialize (H7 _ H11); destruct H7 as [cidx ?].
-          eexists; eapply rsUpMsgOutInv_oinds_tl; eassumption.
-        * eapply downLockCoverInv_oinds_tl; eassumption.
-        * eapply downLockInRoot_oinds_tl; eassumption.
-      + pose proof (downLockCoverInv_DownLockInRoot_NoDownLock
-                      (oinds:= oidx :: oinds)
-                      rsUps H2 (or_introl eq_refl) H6 H7 H8 H9).
-        clear -H11; red in H11.
-        destruct (orqs@[oidx]); [|reflexivity].
-        simpl in *; unfold DownLockNorm.
-        rewrite H11; reflexivity.
-  Qed.
+  (*   induction oinds as [|oidx oinds]; simpl; intros; [exfalso; auto|]. *)
+  (*   destruct H2; dest. *)
+  (*   - clear IHoinds. *)
+  (*     subst; mred; simpl. *)
+  (*     unfold DownLockNorm; repeat (simpl; mred). *)
+  (*     rewrite H6. *)
+  (*     rewrite downLocksNorm_NoDownLocks_zero; [omega|]. *)
+  (*     eapply downLocksNorm_rsUps_NoDownLocks; eauto. *)
+  (*     + intros. *)
+  (*       specialize (H7 _ H2); destruct H7 as [cidx ?]. *)
+  (*       eexists; eapply rsUpMsgOutInv_oinds_tl; eassumption. *)
+  (*     + eapply downLockCoverInv_oinds_tl; eassumption. *)
+  (*     + eapply downLockInRoot_oinds_tl; eassumption. *)
+  (*   - replace ((orqs@[oidx]) >>=[0] (fun orq => DownLockNorm orq)) with 0. *)
+  (*     + simpl; eapply IHoinds. *)
+  (*       * assumption. *)
+  (*       * intros. *)
+  (*         specialize (H7 _ H11); destruct H7 as [cidx ?]. *)
+  (*         eexists; eapply rsUpMsgOutInv_oinds_tl; eassumption. *)
+  (*       * eapply downLockCoverInv_oinds_tl; eassumption. *)
+  (*       * eapply downLockInRoot_oinds_tl; eassumption. *)
+  (*     + pose proof (downLockCoverInv_DownLockInRoot_NoDownLock *)
+  (*                     (oinds:= oidx :: oinds) *)
+  (*                     rsUps H2 (or_introl eq_refl) H6 H7 H8 H9). *)
+  (*       clear -H11; red in H11. *)
+  (*       destruct (orqs@[oidx]); [|reflexivity]. *)
+  (*       simpl in *; unfold DownLockNorm. *)
+  (*       rewrite H11; reflexivity. *)
+  (* Qed. *)
   
   Lemma msgOutsCases_NoDup:
-    forall orqs oinds eouts,
-      MsgOutsCases orqs oinds eouts ->
+    forall oinds orqs1 orqs2 eouts,
+      MsgOutsCases oinds orqs1 orqs2 eouts ->
       NoDup (idsOf eouts).
   Proof.
     intros; inv H.
+    - repeat constructor; auto.
     - repeat constructor; auto.
     - assumption.
   Qed.
@@ -421,101 +590,167 @@ Section MsgOutCases.
   Lemma step_msg_outs_ok:
     forall st1 st2 oidx ridx rins routs,
       Reachable (steps step_m) sys st1 ->
-      NonRqUpL dtr (RlblInt oidx ridx rins routs) ->
       step_m sys st1 (RlblInt oidx ridx rins routs) st2 ->
-      MsgOutsCases st2.(bst_orqs) [oidx] routs.
+      MsgOutsCases [oidx] st1.(bst_orqs) st2.(bst_orqs) routs.
   Proof.
     destruct Hrrs as [? [? ?]]; intros.
     pose proof (footprints_ok H0 H2).
     inv_step.
     good_rqrs_rule_get rule.
-    pose proof H; destruct H6 as [? _].
     good_rqrs_rule_cases rule; simpl in *.
 
     - disc_rule_conds.
-      eapply MsgOutsRsDown; solve_msg_out_cases.
+      eapply MsgOutsRsDown.
+      + split.
+        * red; eauto.
+        * red; intros; Common.dest_in.
+          apply parent_not_in_subtree; [apply Hrrs|]; assumption.
+      + red; intros; Common.dest_in.
+        red; mred.
 
     - disc_rule_conds.
-      eapply MsgOutsRqDownRsUp; solve_msg_out_cases.
-      unfold DownLockNorm; mred.
+      eapply MsgOutsRqDownRsUp.
+      + repeat constructor; auto.
+      + repeat constructor.
+        eexists; right.
+        split; [red; eauto|].
+        red; intros; Common.dest_in.
+        red; mred.
+      + red; intros; Common.dest_in.
+        red; intros.
+        red; apply (DisjList_singleton_1 eq_nat_dec).
+        apply parent_not_in_subtree; [apply Hrrs|]; assumption.
+      + intros; exfalso.
+        red in H3; dest; Common.dest_in.
+        red in H5; mred; simpl in H5; congruence.
 
     - disc_rule_conds.
-      + exfalso.
-        pose proof (rqEdgeUpFrom_Some H _ H8).
-        destruct H15 as [rsUp [down [pidx ?]]]; dest.
-        repeat disc_rule_minds.
-        elim (H3 pidx).
-        do 2 eexists; eauto.
-      + eapply MsgOutsRqDownRsUp; solve_msg_out_cases.
-        * destruct H20; assumption.
+      + eapply MsgOutsRqUp.
+        * do 2 red; eauto.
+        * red; intros; Common.dest_in.
+          red in H20; repeat (simpl in H20; mred).
+          red; intros; apply (DisjList_singleton_1 eq_nat_dec).
+          apply parent_not_in_subtree; [apply Hrrs|]; assumption.
+
+      + eapply MsgOutsRqDownRsUp.
+        * destruct H19; assumption.
         * apply Forall_forall; intros [midx msg] ?.
-          rewrite Forall_forall in H34; specialize (H34 _ H7).
+          rewrite Forall_forall in H32; specialize (H32 _ H5).
+          apply in_map with (f:= idOf) in H5.
+          eapply RqRsDownMatch_rq_rs in H20; [|eassumption].
+          destruct H20 as [cidx [rsUp ?]]; dest.
+          eexists; left.
+          split; [red; eauto|].
+          red; apply (DisjList_singleton_1 eq_nat_dec).
+          apply parent_not_in_subtree; [apply Hrrs|]; assumption.
+        * red; intros; Common.dest_in.
+          red; intros.
+          red; apply (DisjList_singleton_1 eq_nat_dec).
+          apply parent_not_in_subtree; [apply Hrrs|]; assumption.
+        * intros.
+          red in H5; dest; Common.dest_in.
+          red in H14; repeat (simpl in H14; mred).
+          repeat split.
+          { red; intros; Common.dest_in.
+            eapply parent_subtreeIndsOf_self_in; [apply Hrrs|eassumption].
+          }
+          { red; intros; Common.dest_in.
+            apply parent_not_in_subtree; [apply Hrrs|]; assumption.
+          }
+          { red; simpl.
+            destruct (eq_nat_dec _ _); [clear e|exfalso; auto].
+            simpl; unfold DownLockNorm; repeat (mred; simpl).
+            red in H20; dest.
+            assert (length (idsOf routs) > 0)
+              by (destruct (idsOf routs); simpl; [exfalso; auto|omega]).
+            omega.
+          }
+
+      + eapply MsgOutsRqDownRsUp.
+        * destruct H19; assumption.
+        * apply Forall_forall; intros [midx msg] ?.
+          rewrite Forall_forall in H32; specialize (H32 _ H7).
           apply in_map with (f:= idOf) in H7.
-          eapply RqRsDownMatch_rq_rs in H23; [|eassumption].
-          destruct H23 as [cidx [rsUp ?]]; dest.
+          eapply RqRsDownMatch_rq_rs in H6; [|eassumption].
+          destruct H6 as [cidx [rsUp ?]]; dest.
           eexists; left.
-          solve_msg_out_cases.
-        * intro Hx.
-          eapply RqRsDownMatch_rs_rq in H23; [|eassumption].
-          destruct H23 as [cidx [down ?]]; dest.
-          disc_rule_conds; auto.
-        * eapply parent_subtreeIndsOf_self_in;
-            [destruct H; assumption|eassumption].
-        * unfold DownLockNorm; mred; simpl.
-          red in H23; dest.
-          assert (length (idsOf routs) > 0)
-            by (destruct (idsOf routs); simpl; [exfalso; auto|omega]).
-          omega.
-      + eapply MsgOutsRqDownRsUp; solve_msg_out_cases.
-        * destruct H20; assumption.
-        * apply Forall_forall; intros [midx msg] ?.
-          rewrite Forall_forall in H34; specialize (H34 _ H9).
-          apply in_map with (f:= idOf) in H9.
-          eapply RqRsDownMatch_rq_rs in H8; [|eassumption].
-          destruct H8 as [cidx [rsUp ?]]; dest.
-          eexists; left.
-          solve_msg_out_cases.
-        * solve_midx_false.
-        * solve_midx_false.
-        * unfold DownLockNorm; mred; simpl.
-          red in H8; dest.
-          assert (length (idsOf routs) > 0)
-            by (destruct (idsOf routs); simpl; [exfalso; auto|omega]).
-          omega.
+          split; [red; eauto|].
+          red; apply (DisjList_singleton_1 eq_nat_dec).
+          apply parent_not_in_subtree; [apply Hrrs|]; assumption.
+        * red; intros; Common.dest_in.
+          red; intros.
+          red; apply (DisjList_singleton_1 eq_nat_dec).
+          apply parent_not_in_subtree; [apply Hrrs|]; assumption.
+        * intros; exfalso.
+          red in H7; dest; Common.dest_in.
+          red in H11; repeat (simpl in H11; mred).
+          solve_midx_false.
 
     - good_footprint_get (obj_idx obj).
       disc_rule_conds.
-      + eapply MsgOutsRsDown; solve_msg_out_cases.
-      + eapply MsgOutsRsDown; solve_msg_out_cases.
-      + eapply MsgOutsRqDownRsUp; solve_msg_out_cases.
-        unfold DownLockNorm; mred.
+      + eapply MsgOutsRsDown.
+        * split; [red; eauto|].
+          red; intros; Common.dest_in.
+          apply parent_not_in_subtree; [apply Hrrs|]; assumption.
+        * red; intros; Common.dest_in.
+          red; repeat (simpl; mred).
+        
+      + eapply MsgOutsRsDown.
+        * split; [red; eauto|].
+          red; intros; Common.dest_in.
+          apply parent_not_in_subtree; [apply Hrrs|]; assumption.
+        * red; intros; Common.dest_in.
+          red; repeat (simpl; mred).
+        
+      + eapply MsgOutsRqDownRsUp.
+        * repeat constructor; auto.
+        * repeat constructor.
+          eexists; right.
+          split; [red; eauto|].
+          red; intros; Common.dest_in.
+          red; repeat (simpl; mred).
+        * red; intros; Common.dest_in.
+          exfalso; red in H20; repeat (simpl in H20; mred).
+        * intros; exfalso.
+          red in H11; dest; Common.dest_in.
+          red in H20; repeat (simpl in H20; mred).
 
     - disc_rule_conds.
-      eapply MsgOutsRqDownRsUp; solve_msg_out_cases.
-      + destruct H20; assumption.
+      eapply MsgOutsRqDownRsUp.
+      + destruct H19; assumption.
       + apply Forall_forall; intros [midx msg] ?.
-        rewrite Forall_forall in H29; specialize (H29 _ H7).
-        apply in_map with (f:= idOf) in H7.
-        eapply RqRsDownMatch_rq_rs in H23; [|eassumption].
-        destruct H23 as [cidx [rsUp ?]]; dest.
+        rewrite Forall_forall in H27; specialize (H27 _ H5).
+        apply in_map with (f:= idOf) in H5.
+        eapply RqRsDownMatch_rq_rs in H20; [|eassumption].
+        destruct H20 as [cidx [rsUp ?]]; dest.
         eexists; left.
-        solve_msg_out_cases.
-      + intro Hx.
-        eapply RqRsDownMatch_rs_rq in H23; [|eassumption].
-        destruct H23 as [cidx [down ?]]; dest.
-        disc_rule_conds; auto.
-      + apply edgeDownTo_subtreeIndsOf_self_in;
-          [destruct H; assumption|congruence].
-      + unfold DownLockNorm; mred; simpl.
-        red in H23; dest.
-        assert (length (idsOf routs) > 0)
-          by (destruct (idsOf routs); simpl; [exfalso; auto|omega]).
-        omega.
+        split; [red; eauto|].
+        apply (DisjList_singleton_1 eq_nat_dec).
+        apply parent_not_in_subtree; [apply Hrrs|]; assumption.
+      + red; intros; Common.dest_in.
+        red; intros.
+        apply (DisjList_singleton_1 eq_nat_dec).
+        apply parent_not_in_subtree; [apply Hrrs|]; assumption.
+      + intros.
+        red in H5; dest; Common.dest_in.
+        red in H22; repeat (simpl in H22; mred).
+        repeat split.
+        * red; intros; Common.dest_in.
+          eapply parent_subtreeIndsOf_self_in; [apply Hrrs|eassumption].
+        * red; intros; Common.dest_in.
+          apply parent_not_in_subtree; [apply Hrrs|]; assumption.
+        * red; simpl.
+          destruct (eq_nat_dec _ _); [clear e|exfalso; auto].
+          simpl; unfold DownLockNorm; repeat (mred; simpl).
+          red in H20; dest.
+          assert (length (idsOf routs) > 0)
+            by (destruct (idsOf routs); simpl; [exfalso; auto|omega]).
+          omega.
   Qed.
 
   Ltac inv_MsgOutsCases :=
     match goal with
-    | [H: MsgOutsCases _ _ _ |- _] => inv H
+    | [H: MsgOutsCases _ _ _ _ |- _] => inv H
     end;
     repeat
       match goal with
@@ -525,9 +760,11 @@ Section MsgOutCases.
         rewrite Forall_forall in H2;
         let oidx := fresh "oidx" in pose proof (H2 _ H1) as [oidx ?]
       | [H: RqDownMsgOutInv _ _ _ \/ RsUpMsgOutInv _ _ _ _ |- _] => destruct H
+      | [H: RqUpMsgOutInv _ _ |- _] => red in H
       | [H: RsDownMsgOutInv _ _ _ |- _] => destruct H
       | [H: RqDownMsgOutInv _ _ _ |- _] => destruct H
       | [H: RsUpMsgOutInv _ _ _ _ |- _] => destruct H
+      | [H: RqUpMsgFrom _ _ |- _] => disc_rule_conds; solve_midx_false; fail
       | [H: RsDownMsgTo _ _ |- _] => disc_rule_conds; solve_midx_false; fail
       | [H: RqDownMsgTo _ _ |- _] => disc_rule_conds; solve_midx_false; fail
       | [H: RsUpMsgFrom _ _ |- _] => disc_rule_conds; solve_midx_false; fail
@@ -537,8 +774,8 @@ Section MsgOutCases.
     forall orqs oinds eouts,
       Forall (fun eout =>
                 exists oidx,
-                  RqDownMsgOutInv oidx eout oinds \/
-                  RsUpMsgOutInv oidx eout orqs oinds) eouts ->
+                  RqDownMsgOutInv oinds oidx eout \/
+                  RsUpMsgOutInv oinds orqs oidx eout) eouts ->
       Forall (fun eout =>
                 exists oidx,
                   RqDownMsgTo oidx eout \/
@@ -562,7 +799,7 @@ Section MsgOutCases.
         steps step_m sys s1 hst s2 ->
         forall oidx rqdm,
           In rqdm eouts ->
-          RqDownMsgOutInv oidx rqdm (oindsOf hst) ->
+          RqDownMsgOutInv (oindsOf hst) oidx rqdm ->
           forall ooidx orqdm,
             RqDownMsgTo ooidx orqdm ->
             In orqdm eouts -> orqdm <> rqdm ->
@@ -593,7 +830,6 @@ Section MsgOutCases.
     rewrite Forall_forall in H10.
     pose proof (H10 _ H5).
     pose proof (H10 _ H8).
-    
     pose proof (downLockInv_ok H0 H (reachable_steps H3 H4)).
     good_locking_get pobj.
     eapply downLockInvORq_down_rqsQ_length_two_False;
@@ -611,7 +847,7 @@ Section MsgOutCases.
         steps step_m sys s1 hst s2 ->
         forall oidx rqdm,
           In rqdm eouts ->
-          RqDownMsgOutInv oidx rqdm (oindsOf hst) ->
+          RqDownMsgOutInv (oindsOf hst) oidx rqdm ->
           forall ooidx opidx opobj orsum,
             parentIdxOf dtr ooidx = Some opidx ->
             In opobj sys.(sys_objs) ->
@@ -643,7 +879,7 @@ Section MsgOutCases.
         steps step_m sys s1 hst s2 ->
         forall oidx rsum,
           In rsum eouts ->
-          RsUpMsgOutInv oidx rsum s2.(bst_orqs) (oindsOf hst) ->
+          RsUpMsgOutInv (oindsOf hst) s2.(bst_orqs) oidx rsum ->
           forall ooidx orqdm,
             RqDownMsgTo ooidx orqdm ->
             In orqdm eouts ->
@@ -696,7 +932,7 @@ Section MsgOutCases.
         steps step_m sys s1 hst s2 ->
         forall oidx rsum,
           In rsum eouts ->
-          RsUpMsgOutInv oidx rsum s2.(bst_orqs) (oindsOf hst) ->
+          RsUpMsgOutInv (oindsOf hst) s2.(bst_orqs) oidx rsum ->
           forall ooidx opidx opobj orsum,
             parentIdxOf dtr ooidx = Some opidx ->
             In opobj sys.(sys_objs) ->
@@ -913,63 +1149,63 @@ Section MsgOutCases.
         rewrite H7 in H37; discriminate.
   Qed.
 
-  Lemma rsUpMsgOutInv_parent_not_in:
-    forall inits ins hst outs eouts,
-      Atomic msg_dec inits ins hst outs eouts ->
-      forall s1 s2,
-        Reachable (steps step_m) sys s1 ->
-        steps step_m sys s1 hst s2 ->
-        MsgOutsNormInv s2.(bst_orqs) (oindsOf hst) eouts ->
-        forall oidx rsUp pidx,
-          In rsUp eouts ->
-          RsUpMsgOutInv oidx rsUp s2.(bst_orqs) (oindsOf hst) ->
-          parentIdxOf dtr oidx = Some pidx ->
-          ~ In pidx (oindsOf hst) ->
-          NoDownLocks (oindsOf hst) (bst_orqs s2) /\
-          SubList (oindsOf hst) (subtreeIndsOf dtr oidx) /\
-          eouts = [rsUp].
-  Proof.
-    intros; red in H2.
-    destruct H4.
-    disc_rule_conds.
-    eapply atomic_non_visiting_rsUp_one in H; try eassumption.
-    assert (NoDownLocks (oindsOf hst) (bst_orqs s2)).
-    { red; intros; eauto. }
-    repeat split; try assumption.
-    rewrite downLocksNorm_NoDownLocks_zero in H2 by assumption.
-    simpl in H2.
-    destruct eouts as [|eout eouts]; [exfalso; auto|].
-    destruct eouts; [|discriminate].
-    Common.dest_in; reflexivity.
-  Qed.
+  (* Lemma rsUpMsgOutInv_parent_not_in: *)
+  (*   forall inits ins hst outs eouts, *)
+  (*     Atomic msg_dec inits ins hst outs eouts -> *)
+  (*     forall s1 s2, *)
+  (*       Reachable (steps step_m) sys s1 -> *)
+  (*       steps step_m sys s1 hst s2 -> *)
+  (*       MsgOutsNormInv s2.(bst_orqs) (oindsOf hst) eouts -> *)
+  (*       forall oidx rsUp pidx, *)
+  (*         In rsUp eouts -> *)
+  (*         RsUpMsgOutInv oidx rsUp s2.(bst_orqs) (oindsOf hst) -> *)
+  (*         parentIdxOf dtr oidx = Some pidx -> *)
+  (*         ~ In pidx (oindsOf hst) -> *)
+  (*         NoDownLocks (oindsOf hst) (bst_orqs s2) /\ *)
+  (*         SubList (oindsOf hst) (subtreeIndsOf dtr oidx) /\ *)
+  (*         eouts = [rsUp]. *)
+  (* Proof. *)
+  (*   intros; red in H2. *)
+  (*   destruct H4. *)
+  (*   disc_rule_conds. *)
+  (*   eapply atomic_non_visiting_rsUp_one in H; try eassumption. *)
+  (*   assert (NoDownLocks (oindsOf hst) (bst_orqs s2)). *)
+  (*   { red; intros; eauto. } *)
+  (*   repeat split; try assumption. *)
+  (*   rewrite downLocksNorm_NoDownLocks_zero in H2 by assumption. *)
+  (*   simpl in H2. *)
+  (*   destruct eouts as [|eout eouts]; [exfalso; auto|]. *)
+  (*   destruct eouts; [|discriminate]. *)
+  (*   Common.dest_in; reflexivity. *)
+  (* Qed. *)
 
-  Lemma rsUpMsgOutInv_parent_not_in_MsgOutsCases:
-    forall inits ins hst outs eouts,
-      Atomic msg_dec inits ins hst outs eouts ->
-      forall s1 s2,
-        Reachable (steps step_m) sys s1 ->
-        steps step_m sys s1 hst s2 ->
-        forall orqs oinds oidx rsUp pidx,
-          orqs = s2.(bst_orqs) -> oinds = oindsOf hst ->
-          In rsUp eouts ->
-          parentIdxOf dtr oidx = Some pidx ->
-          ~ In pidx (oindsOf hst) ->
-          RsUpMsgOutInv oidx rsUp orqs oinds ->
-          MsgOutsNormInv orqs oinds eouts ->
-          MsgOutsCases orqs oinds eouts.
-  Proof.
-    intros; subst.
-    eapply rsUpMsgOutInv_parent_not_in in H6; try eassumption.
-    dest; subst; clear H4.
-    eapply MsgOutsRqDownRsUp; eauto.
-    - repeat constructor; auto.
-    - red; intros; exfalso.
-      specialize (H2 _ H4).
-      red in H2; mred.
-    - red; intros; exfalso.
-      specialize (H2 _ H4).
-      red in H2; mred.
-  Qed.
+  (* Lemma rsUpMsgOutInv_parent_not_in_MsgOutsCases: *)
+  (*   forall inits ins hst outs eouts, *)
+  (*     Atomic msg_dec inits ins hst outs eouts -> *)
+  (*     forall s1 s2, *)
+  (*       Reachable (steps step_m) sys s1 -> *)
+  (*       steps step_m sys s1 hst s2 -> *)
+  (*       forall orqs oinds oidx rsUp pidx, *)
+  (*         orqs = s2.(bst_orqs) -> oinds = oindsOf hst -> *)
+  (*         In rsUp eouts -> *)
+  (*         parentIdxOf dtr oidx = Some pidx -> *)
+  (*         ~ In pidx (oindsOf hst) -> *)
+  (*         RsUpMsgOutInv oidx rsUp orqs oinds -> *)
+  (*         MsgOutsNormInv orqs oinds eouts -> *)
+  (*         MsgOutsCases orqs oinds eouts. *)
+  (* Proof. *)
+  (*   intros; subst. *)
+  (*   eapply rsUpMsgOutInv_parent_not_in in H6; try eassumption. *)
+  (*   dest; subst; clear H4. *)
+  (*   eapply MsgOutsRqDownRsUp; eauto. *)
+  (*   - repeat constructor; auto. *)
+  (*   - red; intros; exfalso. *)
+  (*     specialize (H2 _ H4). *)
+  (*     red in H2; mred. *)
+  (*   - red; intros; exfalso. *)
+  (*     specialize (H2 _ H4). *)
+  (*     red in H2; mred. *)
+  (* Qed. *)
 
   Section InternalStep.
 
@@ -983,16 +1219,18 @@ Section MsgOutCases.
     Hypotheses
       (Hatm: Atomic msg_dec inits ins hst outs eouts)
       (Hrch: Reachable (steps step_m) sys st0)
-      (Hsteps: steps step_m sys st0 hst {| bst_oss := oss; bst_orqs := orqs; bst_msgs := msgs |})
+      (Hsteps: steps step_m sys st0 hst {| bst_oss := oss;
+                                           bst_orqs := orqs;
+                                           bst_msgs := msgs |})
       (Hrins: rins <> nil)
       (Hosub: SubList rins eouts)
-      (Hmoc: MsgOutsCases orqs (oindsOf hst) eouts)
-      (* (Hnruh: Forall (NonRqUpL dtr) hst) *)
-      (* (Hnrul: NonRqUpL dtr (RlblInt (obj_idx obj) (rule_idx rule) rins routs)) *)
-      (Hnrul: Forall (fun eout : Id Msg =>
-                        forall oidxTo, ~ RqUpMsgs dtr oidxTo [eout]) rins)
-      (Hftinv: FootprintsOk dtr sys {| bst_oss := oss; bst_orqs := orqs; bst_msgs := msgs |})
-      (Hdlinv: DownLockInv dtr sys {| bst_oss := oss; bst_orqs := orqs; bst_msgs := msgs |})
+      (Hmoc: MsgOutsCases (oindsOf hst) st0.(bst_orqs) orqs eouts)
+      (Hftinv: FootprintsOk dtr sys {| bst_oss := oss;
+                                       bst_orqs := orqs;
+                                       bst_msgs := msgs |})
+      (Hdlinv: DownLockInv dtr sys {| bst_oss := oss;
+                                      bst_orqs := orqs;
+                                      bst_msgs := msgs |})
       (Hnodup:
          forall pobj,
            In pobj sys.(sys_objs) ->
@@ -1021,741 +1259,734 @@ Section MsgOutCases.
 
     Lemma step_msg_outs_ok_ImmDownRule:
       ImmDownRule dtr (obj_idx obj) rule ->
-      MsgOutsCases (orqs +[obj_idx obj <- norq])
-                   (obj_idx obj :: oindsOf hst)
+      MsgOutsCases (obj_idx obj :: oindsOf hst)
+                   st0.(bst_orqs) (orqs +[obj_idx obj <- norq])
                    (removeL (id_dec msg_dec) eouts rins ++ routs).
     Proof.
-      intros.
-      disc_rule_conds.
-      elim (H9 (obj_idx obj)).
-      do 2 eexists; eauto.
-    Qed.
-
-    Lemma step_msg_outs_ok_ImmUpRule:
-      ImmUpRule dtr (obj_idx obj) rule ->
-      MsgOutsCases (orqs +[obj_idx obj <- norq])
-                   (obj_idx obj :: oindsOf hst)
-                   (removeL (id_dec msg_dec) eouts rins ++ routs).
-    Proof.
-      destruct Hrrs as [? [? ?]]; intros.
-      disc_rule_conds.
-      replace (orqs+[obj_idx obj <- norq]) with orqs by meq.
-
-      inv_MsgOutsCases.
-
-      pose proof (edgeDownTo_Some H _ H11).
-      destruct H15 as [rqUp [rsUp [pidx ?]]]; dest.
-      disc_rule_conds.
-      assert (In rqFrom (idsOf eouts))
-        by (apply in_map_iff; exists (rqFrom, rqm); auto).
-      pose proof (atomic_down_out_in_history
-                    Hrrs Hatm Hrch Hsteps _ H11 H18 H16); clear H16.
-
-      eapply MsgOutsRqDownRsUp.
-      - pose proof (steps_object_in_system Hsteps _ H19).
-        destruct H16 as [pobj [? ?]]; subst.
-        eapply Hnodup with (pobj0:= pobj).
-        + assumption.
-        + reflexivity.
-        + eapply rqDown_rsUp_inv_msg.
-          rewrite Forall_forall; eassumption.
-        + repeat constructor.
-          exists (obj_idx obj); right.
-          red; auto.
-
-      - (* Invariant for each message *)
-        apply Forall_app.
-        + (* For the others except (rqFrom, rqm) *)
-          apply Forall_forall.
-          intros [midx msg] ?.
-          apply removeOnce_In_NoDup in H16;
-            [|apply idsOf_NoDup; assumption]; dest.
-
-          pose proof (H3 _ H20).
-          destruct H21 as [oidx ?].
-          destruct H21.
-          * (* RqDown *)
-            exists oidx; left.
-            destruct H21.
-            split; [assumption|].
-            red in H22.
-            red; simpl.
-            apply (DisjList_cons_inv eq_nat_dec); [assumption|].
-
-            eapply rqDownMsgOutInv_no_rqDown
-              with (oidx := oidx) (rqdm := (midx, msg))
-                   (ooidx := obj_idx obj) (orqdm := (rqFrom, rqm));
-              try eassumption.
-            { split; assumption. }
-            { split; assumption. }
-            { congruence. }
-          * (* RsUp *)
-            exists oidx; right.
-            destruct H21.
-            split; [assumption|].
-            red; simpl; intros.
-            destruct H23; [subst|auto].
-            red; mred.
-          
-        + (* For the new output *)
-          repeat constructor.
-          exists (obj_idx obj); right.
-          split; [red; auto|].
-          red; simpl; intros.
-          destruct H16.
-          * subst; red; mred.
-          * specialize (H14 oidx); destruct H14; exfalso; auto.
-          
-      - red; simpl; intros.
-        destruct H16; [subst; mred|].
-        red; intros.
-        red; simpl.
-        apply (DisjList_cons_inv eq_nat_dec);
-          [eapply H5; eauto|].
-
-        intro Hx.
-        specialize (H5 _ _ _ H16 H20 H21 _ _ H22 H23 H24).
-        red in H5.
-        eapply DisjList_In_2 in H19; [|eapply H5].
-        eapply inside_child_outside_parent_case in Hx;
-          try eassumption; try apply Hrrs; subst.
-
-        pose proof (steps_object_in_system Hsteps _ H16).
-        destruct H25 as [dobj [? ?]]; subst.
-        good_locking_get dobj; mred.
-        red in H26; mred.
-
-        disc_rule_conds.
-        specialize (H26 _ H18).
-        destruct H26 as [down [rsUp ?]]; dest.
-        disc_rule_conds.
-        destruct (in_dec eq_nat_dec rsUp _); [auto|].
-        red in H26; dest.
-        eapply rqsQ_length_zero_False; eauto.
-        
-      - red; simpl; intros.
-        destruct H16; [subst; mred|].
-        pose proof (H8 _ _ _ _ _ H16 H20 H21 H22 H23 H24); dest.
-        repeat ssplit; [assumption| |].
-        + red in H27.
-          red; simpl.
-          apply (DisjList_cons_inv eq_nat_dec); [auto|].
-          intro Hx.
-          eapply DisjList_In_2 in H19; [|eassumption].
-          eapply inside_child_outside_parent_case in Hx;
-            try eassumption; try apply Hrrs; subst.
-          disc_rule_conds.
-
-          pose proof (steps_object_in_system Hsteps _ H16).
-          destruct H22 as [robj [? ?]]; subst.
-          good_locking_get robj; mred.
-          red in H23; mred.
-          specialize (H23 _ H18).
-          destruct H23 as [down [rsUp' ?]]; dest.
-          disc_rule_conds.
-          destruct (in_dec eq_nat_dec rsUp' _); [auto|].
-          red in H28; dest.
-          eapply rqsQ_length_zero_False; eauto.
-        + red; simpl; intros.
-          destruct H28; [subst|eauto].
-          mred.
-
-      - red; repeat (simpl; mred).
-        rewrite idsOf_app; simpl.
-        rewrite app_length; simpl.
-        unfold idsOf; rewrite map_length.
-        pose proof (removeOnce_length (id_dec msg_dec) _ _ Hosub); dest.
-        unfold Id in *; rewrite H20.
-        unfold DownLockNorm; repeat (simpl; mred).
-        red in H10.
-        unfold idsOf in H10; rewrite map_length in H10.
-        omega.
-    Qed.
-
-    Lemma step_msg_outs_ok_RqFwdRule:
-      RqFwdRule dtr sys (obj_idx obj) rule ->
-      MsgOutsCases (orqs +[obj_idx obj <- norq])
-                   (obj_idx obj :: oindsOf hst)
-                   (removeL (id_dec msg_dec) eouts rins ++ routs).
-    Proof.
-      destruct Hrrs as [? [? ?]]; intros.
-      disc_rule_conds.
-      { elim (H19 (obj_idx obj)); do 2 eexists; eauto. }
-      { elim (H17 (obj_idx obj)); do 2 eexists; eauto. }
-
-      inv_MsgOutsCases.
-      pose proof (edgeDownTo_Some H _ H2).
-      destruct H19 as [rqUp [rsUp [pidx ?]]]; dest.
-      disc_rule_conds.
-      assert (In rqFrom (idsOf eouts))
-        by (apply in_map_iff; exists (rqFrom, rqi_msg rqi); auto).
-      pose proof (atomic_down_out_in_history
-                    Hrrs Hatm Hrch Hsteps _ H2 H22 H21); clear H21.
-
-      eapply MsgOutsRqDownRsUp.
-      - pose proof (steps_object_in_system Hsteps _ H23).
-        destruct H21 as [pobj [? ?]]; subst.
-        eapply Hnodup with (pobj0:= pobj).
-        + assumption.
-        + reflexivity.
-        + eapply rqDown_rsUp_inv_msg.
-          rewrite Forall_forall; eassumption.
-        + apply Forall_forall.
-          intros [rqDown rqm] ?.
-          rewrite Forall_forall in H20; specialize (H20 _ H24).
-          apply in_map with (f:= idOf) in H24; simpl in H24.
-          eapply RqRsDownMatch_rq_rs in H4; [|eassumption].
-          destruct H4 as [cidx [rsUp ?]]; dest.
-          exists cidx; left.
-          red; auto.
-
-      - apply Forall_app.
-        + apply Forall_forall.
-          intros [midx msg] ?.
-          apply removeOnce_In_NoDup in H21;
-            [|apply idsOf_NoDup; assumption]; dest.
-
-          pose proof (H7 _ H24).
-          destruct H25 as [oidx ?].
-          destruct H25.
-          * (* RqDown *)
-            exists oidx; left.
-            destruct H25.
-            split; [assumption|].
-            red in H26.
-            red; simpl.
-            apply (DisjList_cons_inv eq_nat_dec); [assumption|].
-
-            eapply rqDownMsgOutInv_no_rqDown
-              with (oidx := oidx) (rqdm := (midx, msg))
-                   (ooidx := obj_idx obj) (orqdm := (rqFrom, rqi_msg rqi));
-              try eassumption.
-            { split; assumption. }
-            { split; assumption. }
-            { congruence. }
-          * (* RsUp *)
-            exists oidx; right.
-            destruct H25.
-            split; [assumption|].
-
-            red; simpl; intros.
-            destruct (eq_nat_dec (obj_idx obj) oidx0).
-            { subst; exfalso.
-              eapply rsUpMsgOutInv_no_rqDown
-                with (oidx := oidx) (rsum := (midx, msg))
-                     (ooidx := obj_idx obj) (orqdm := (rqFrom, rqi_msg rqi));
-                try eassumption.
-              { split; assumption. }
-              { split; assumption. }
-            }
-            { destruct H27; [exfalso; auto|].
-              specialize (H26 _ H27 H28).
-              red; mred.
-            }
-
-        + apply Forall_forall.
-          intros [rqTo rqm] ?.
-          assert (In rqTo (idsOf routs))
-            by (apply in_map_iff; exists (rqTo, rqm); auto).
-          eapply RqRsDownMatch_rq_rs in H4; [|eassumption].
-          destruct H4 as [cidx [rsUp ?]]; dest.
-          rewrite Forall_forall in H20.
-          pose proof (H20 _ H21); simpl in H29.
-          exists cidx; left.
-          split; [red; auto|].
-          red in H18; red; simpl.
-          apply (DisjList_cons_inv eq_nat_dec).
-          { apply DisjList_comm in H18.
-            eapply DisjList_comm, DisjList_SubList;
-              [|eassumption].
-            eapply subtreeIndsOf_child_SubList;
-              [apply Hrrs|assumption].
-          }
-          { apply parent_not_in_subtree; [apply Hrrs|auto]. }
-
-      - red; simpl; intros.
-        destruct (eq_nat_dec (obj_idx obj) oidx).
-        + subst; mred.
-          red; intros.
-          red in H18; red; simpl.
-          apply (DisjList_cons_inv eq_nat_dec).
-          * eapply DisjList_comm in H18.
-            eapply DisjList_comm, DisjList_SubList; [|eassumption].
-            apply subtreeIndsOf_child_SubList;
-              [apply Hrrs|assumption].
-          * eapply parent_not_in_subtree; [apply Hrrs|auto].
-        + destruct H21; [exfalso; auto|].
-          mred; specialize (H11 _ _ _ H21 H24 H25).
-          red; intros.
-          specialize (H11 _ _ H26 H27 H28).
-          red in H11.
-          red; simpl; intros.
-          apply (DisjList_cons_inv eq_nat_dec); [assumption|].
-          eapply DisjList_In_2 in H23; [|eapply H11].
-          eapply outside_child_in in H23; try apply Hrrs; [|eassumption].
-          destruct H23; [subst; exfalso|assumption].
-          pose proof (steps_object_in_system Hsteps _ H21).
-          destruct H23 as [oobj [? ?]]; subst.
-          good_locking_get oobj.
-          red in H29; mred.
-
-          disc_rule_conds.
-          specialize (H29 _ H22).
-          destruct H29 as [down [rsUp ?]]; dest.
-          disc_rule_conds.
-          destruct (in_dec eq_nat_dec (rqi_midx_rsb rqi) _); [auto|].
-          red in H29; dest.
-          eapply rqsQ_length_zero_False; eauto.
-          
-      - red; simpl; intros.
-        destruct (eq_nat_dec (obj_idx obj) roidx);
-          [subst; exfalso; mred; solve_midx_false|].
-        destruct H21; [exfalso; auto|].
-        mred.
-        specialize (H13 _ _ _ _ _ H21 H24 H25 H26 H27 H28); dest.
-        repeat ssplit; [assumption| |].
-        + red in H29.
-          red; simpl.
-          apply (DisjList_cons_inv eq_nat_dec); [auto|].
-          intro Hx.
-          eapply DisjList_In_2 in H23; [|apply H29].
-          eapply inside_child_outside_parent_case in Hx;
-            try eassumption; try apply Hrrs; subst.
-          disc_rule_conds.
-
-          pose proof (steps_object_in_system Hsteps _ H21).
-          destruct H26 as [robj [? ?]]; subst.
-          good_locking_get robj; mred.
-          red in H27; mred.
-          specialize (H27 _ H22).
-          destruct H27 as [down [rsUp ?]]; dest.
-          disc_rule_conds.
-          destruct (in_dec eq_nat_dec (rqi_midx_rsb rqi) _); [auto|].
-          red in H31; dest.
-          eapply rqsQ_length_zero_False; eauto.
-        + red; simpl; intros.
-          destruct (eq_nat_dec (obj_idx obj) sidx).
-          * subst; clear H31; mred.
-            pose proof (steps_object_in_system Hsteps _ H23).
-            destruct H31 as [pobj [? ?]]; subst.
-            good_locking_get pobj.
-            eapply downLockInvORq_down_rqsQ_length_one_locked in H32;
-              try eassumption;
-              [|eapply rqsQ_length_ge_one;
-                [eassumption|apply FirstMP_InMP; assumption]].
-            destruct H32 as [prqid ?]; dest.
-            remember (orqs@[obj_idx pobj]) as pporq; apply eq_sym in Heqpporq.
-            destruct pporq as [pporq|]; [simpl in H32|discriminate].
-            eapply inside_child_in; [apply Hrrs|eassumption|].
-            eapply H30; eassumption.
-          * destruct H31; [exfalso; auto|].
-            mred; eauto.
-        
-      - red; repeat (simpl; mred).
-        rewrite idsOf_app; simpl.
-        rewrite app_length; simpl.
-        unfold idsOf; rewrite map_length.
-        pose proof (removeOnce_length (id_dec msg_dec) _ _ Hosub); dest.
-        unfold Id in *; rewrite H24.
-        unfold DownLockNorm; repeat (simpl; mred).
-
-        red in H4; dest; rewrite <-H25.
-        rewrite downLocksNorm_orqs_add.
-        + assert (length (idsOf routs) > 0)
-            by (destruct (idsOf routs); [exfalso; auto|simpl; omega]).
-          red in H15.
-          unfold idsOf in H15; rewrite map_length in H15.
-          rewrite H15.
-          unfold idsOf in *.
-          omega.
-        + specialize (H7 _ Hosub).
-          destruct H7 as [oidx ?].
-          destruct H7; [|destruct H7; disc_rule_conds].
-          destruct H7; disc_rule_conds.
-          red in H18.
-          eapply DisjList_In_1.
-          * eassumption.
-          * apply rsEdgeUpFrom_subtreeIndsOf_self_in; [apply Hrrs|congruence].
-    Qed.
-
-    Lemma step_msg_outs_ok_RsBackRule:
-      RsBackRule rule ->
-      MsgOutsCases (orqs +[obj_idx obj <- norq])
-                   (obj_idx obj :: oindsOf hst)
-                   (removeL (id_dec msg_dec) eouts rins ++ routs).
-    Proof.
-      destruct Hrrs as [? [? ?]]; intros.
-      good_footprint_get (obj_idx obj).
-      disc_rule_conds.
-      - (** [RsDownDown] *)
-        inv_MsgOutsCases.
-        disc_rule_conds.
-        destruct (id_dec msg_dec i i) as [_|]; [simpl|exfalso; auto].
-
-        eapply MsgOutsRsDown.
-        + split; [red; simpl; eauto|].
-          red; simpl.
-          apply (DisjList_cons_inv eq_nat_dec).
-          * red in H16; apply DisjList_comm in H16.
-            eapply DisjList_comm, DisjList_SubList; [|eassumption].
-            apply subtreeIndsOf_child_SubList; [apply Hrrs|assumption].
-          * apply parent_not_in_subtree; [apply Hrrs|assumption].
-        + red; simpl; intros.
-          destruct H18; subst.
-          * red; repeat (simpl; mred).
-          * specialize (H15 _ H18).
-            red in H15; red.
-            repeat (simpl; mred).
-
-      - (** [RsUpDown] *)
-        inv_MsgOutsCases.
-        + exfalso.
-          eapply SubList_singleton_NoDup in Hosub;
-            [|apply idsOf_NoDup, HminsV].
-          destruct Hosub; [exfalso; auto|subst].
-          rewrite <-H17 in H10.
-          eapply RqRsDownMatch_rs_rq in H10; [|left; reflexivity].
-          destruct H10 as [cidx [down ?]]; dest.
-          disc_rule_conds.
-          solve_midx_false.
-
-        + pose proof (edgeDownTo_Some H _ H9).
-          destruct H18 as [rqUp [rsUp [pidx ?]]]; dest.
-          disc_rule_conds.
-          rewrite Forall_forall in H11.
-
-          (* Different proofs whether the object is part of the history or not *)
-          destruct (in_dec eq_nat_dec (obj_idx obj) (oindsOf hst)).
-          * (* If the object is in the history, we can use 1) [DownLockRootInv]
-             * to say all downlocks are in the tree of the object and 2) the RsUp
-             * invariants to say there are no downlocks in the tree.
-             *)
-            specialize (H15 _ _ _ _ _ i Hporq H14 H5 H9 H19); dest.
-            specialize (H13 _ _ _ i Hporq H14).
-            assert (removeL (id_dec msg_dec) eouts rins = nil).
-            { eapply SubList_NoDup_length_eq_removeL_nil.
-              { assumption. }
-              { apply idsOf_NoDup, HminsV. }
-              { (* [length rins = length eouts] *)
-                (** FIXME: must use [downLocksNorm_rsUps] here, but it requires
-                 * strengthening the invariant about the RsDown-root to appear
-                 * at most once in the history.
-                 *)
-                admit.
-              }
-            }
-            rewrite H21; simpl; clear H21.
-            
-            eapply MsgOutsRsDown.
-            { split; [red; eauto|].
-              red; simpl.
-              apply (DisjList_cons_inv eq_nat_dec); [assumption|].
-              apply parent_not_in_subtree; [apply Hrrs|assumption].
-            }
-            { simpl; red; simpl; intros.
-              destruct (eq_nat_dec (obj_idx obj) oidx);
-                [subst; red; repeat (simpl; mred)|].
-              destruct H21; [exfalso; auto|].
-              eapply downLockCoverInv_DownLockInRoot_NoDownLock with (ridx:= obj_idx obj).
-              { auto. }
-              { eassumption. }
-              { apply eq_sym; eassumption. }
-              { intros [rrsUp rrsm] ?.
-                rewrite <-H17 in H10.
-                assert (In rrsUp (idsOf rins))
-                  by (apply in_map with (f:= idOf) in H22; assumption).
-                eapply RqRsDownMatch_rs_rq in H10; [|eassumption]; clear H23.
-                destruct H10 as [rcidx [rdown ?]]; dest.
-                apply Hosub in H22.
-                specialize (H11 _ H22).
-                destruct H11 as [cidx ?].
-                destruct H11; [destruct H11; disc_rule_conds; solve_midx_false|].
-                exists cidx.
-                apply rsUpMsgOutInv_orqs_downRq_remove; assumption.
-              }
-              { assumption. }
-              { apply downLockInRoot_orqs_downRq_remove; assumption. }
-            }
-
-          * (* When [~ In (obj_idx obj) (oindsOf hst)] *)
-            admit.
-
-      - (** [RsUpUp] *)
-        inv_MsgOutsCases.
-        { exfalso.
-          eapply SubList_singleton_NoDup in Hosub;
-            [|apply idsOf_NoDup, HminsV].
-          destruct Hosub; [exfalso; auto|subst].
-          rewrite <-H17 in H5.
-          eapply RqRsDownMatch_rs_rq in H5; [|left; reflexivity].
-          destruct H5 as [cidx [down ?]]; dest.
-          disc_rule_conds.
-          solve_midx_false.
-        }
-
-        pose proof (edgeDownTo_Some H _ H2).
-        destruct H15 as [rqUp [rsUp [pidx ?]]]; dest.
-        rewrite Forall_forall in H9.
-        disc_rule_conds.
-
-        (* Different proofs whether the object is part of the history or not *)
-        destruct (in_dec eq_nat_dec (obj_idx obj) (oindsOf hst)).
-        + (* Need to have just one child of the incoming RsUp messages. *)
-          assert (exists rsFrom rsfm, In (rsFrom, rsfm) rins).
-          { destruct rins as [|[rsFrom rsfm] ?]; [exfalso; auto|].
-            do 2 eexists; left; reflexivity.
-          }
-          destruct H16 as [rsFrom [rsfm ?]].
-          rewrite Forall_forall in H8.
-          specialize (H8 _ H16); simpl in H8.
-          assert (In rsFrom (idsOf rins))
-            by (apply in_map with (f:= idOf) in H16; assumption).
-          rewrite <-H17 in H5.
-          eapply RqRsDownMatch_rs_rq in H5; [|eassumption]; clear H19.
-          destruct H5 as [ccidx [down ?]]; dest.
-          eapply Hosub in H16.
-          assert (In rsFrom (idsOf eouts))
-            by (apply in_map with (f:= idOf) in H16; assumption).
-          pose proof (atomic_rsUp_out_in_history
-                        Hrrs Hatm Hrch Hsteps _ H21 H23); clear H23.
-
-          eapply MsgOutsRqDownRsUp.
-          * (* [NoDup] for [RsUpUp] *)
-            eapply Hnodup.
-            { admit. }
-            { admit. }
-            { eapply rqDown_rsUp_inv_msg.
-              rewrite Forall_forall; eassumption.
-            }
-            { repeat constructor.
-              exists (obj_idx obj); right.
-              red; auto.
-            }
-
-          * apply Forall_app.
-            { apply Forall_forall.
-              intros [midx msg] ?.
-              apply removeL_In_NoDup in H23; [|apply idsOf_NoDup; assumption]; dest.
-              pose proof (H9 _ H25).
-              destruct H26 as [oidx ?]; destruct H26.
-              { exists oidx; left.
-                destruct H26.
-                split; [assumption|].
-                red; simpl.
-                apply (DisjList_cons_inv eq_nat_dec); [auto|].
-                eapply rqDownMsgOutInv_no_rsUp with (orsum := (rsFrom, rsfm));
-                  try eassumption.
-                { split; assumption. }
-                { reflexivity. }
-                { red; auto. }
-              }
-              { exists oidx; right.
-                destruct H26.
-                split; [assumption|].
-                red; simpl; intros.
-                destruct (eq_nat_dec (obj_idx obj) oidx0);
-                  [subst; red; repeat (simpl; mred)|].
-                destruct H28; [exfalso; auto|].
-                red; mred.
-                eapply H27; eauto.
-              }
-            }
-            { repeat constructor.
-              exists (obj_idx obj); right.
-              split; [red; auto|].
-              red; simpl; intros.
-              destruct (eq_nat_dec (obj_idx obj) oidx);
-                [subst; red; repeat (simpl; mred)|].
-              destruct H23; [exfalso; auto|].
-              red; mred.
-              apply subtreeIndsOf_composed in H25; [|apply Hrrs].
-              destruct H25; [exfalso; auto|].
-              destruct H25 as [cidx [? ?]].
-              pose proof (parentIdxOf_Some H _ H25).
-              destruct H27 as [crqUp [crsUp [cdown ?]]]; dest.
-              destruct (in_dec eq_nat_dec crsUp rqi.(rqi_minds_rss)).
-              { rewrite <-H17 in i0.
-                apply in_map_iff in i0.
-                destruct i0 as [[crsUp' crsm] [? ?]]; simpl in *; subst.
-                apply Hosub in H31.
-                specialize (H9 _ H31).
-                destruct H9 as [rcidx ?].
-                destruct H9; [destruct H9; disc_rule_conds; solve_midx_false|].
-                destruct H9; disc_rule_conds.
-                specialize (H30 _ H23 H26).
-                red in H30; destruct (orqs@[oidx]); auto.
-              }
-              { specialize (H10 _ _ _ i Hporq H14).
-                red in H10.
-                specialize (H10 _ _ H25 H28 n0 oidx).
-                exfalso; destruct H10; eauto.
-              }
-            }
-
-          * red; simpl; intros.
-            destruct (eq_nat_dec (obj_idx obj) oidx);
-              [subst; red; repeat (simpl; mred)|].
-            destruct H23; [exfalso; auto|].
-            mred; red; intros.
-            red; simpl; intros.
-            apply (DisjList_cons_inv eq_nat_dec); [eapply H10; eauto|].
-            specialize (H10 _ _ _ H23 H25 H26).
-            specialize (H10 _ _ H27 H28 H29).
-            eapply outside_parent_out; [apply Hrrs| |eassumption].
-            eapply DisjList_In_2; eassumption.
-
-          * red; simpl; intros.
-            destruct (eq_nat_dec (obj_idx obj) roidx); [subst; mred|].
-            destruct H23; [exfalso; auto|].
-            mred.
-            specialize (H11 _ _ _ _ _ H23 H25 H26 H27 H28 H29); dest.
-            repeat split; [assumption| |].
-            { red; simpl.
-              apply (DisjList_cons_inv eq_nat_dec); [auto|].
-              eapply outside_parent_out; [apply Hrrs| |eassumption].
-              eapply DisjList_In_2; eassumption.
-            }
-            { red; simpl; intros.
-              destruct (eq_nat_dec (obj_idx obj) sidx); [subst; mred|].
-              destruct H32; [exfalso; auto|].
-              mred; eauto.
-            }
-
-          * red; repeat (simpl; mred).
-            rewrite idsOf_app, app_length; simpl.
-            unfold DownLockNorm; repeat (simpl; mred).
-            (* [MsgOutsNormInv] for [RsUpUp] *)
-            admit.
-
-        + (* When [~ In (obj_idx obj) (oindsOf hst)] *)
-          admit.
-            
     Admitted.
+
+    (*   Lemma step_msg_outs_ok_ImmUpRule: *)
+    (*     ImmUpRule dtr (obj_idx obj) rule -> *)
+    (*     MsgOutsCases (orqs +[obj_idx obj <- norq]) *)
+    (*                  (obj_idx obj :: oindsOf hst) *)
+    (*                  (removeL (id_dec msg_dec) eouts rins ++ routs). *)
+    (*   Proof. *)
+    (*     destruct Hrrs as [? [? ?]]; intros. *)
+    (*     disc_rule_conds. *)
+    (*     replace (orqs+[obj_idx obj <- norq]) with orqs by meq. *)
+
+    (*     inv_MsgOutsCases. *)
+
+    (*     pose proof (edgeDownTo_Some H _ H11). *)
+    (*     destruct H15 as [rqUp [rsUp [pidx ?]]]; dest. *)
+    (*     disc_rule_conds. *)
+    (*     assert (In rqFrom (idsOf eouts)) *)
+    (*       by (apply in_map_iff; exists (rqFrom, rqm); auto). *)
+    (*     pose proof (atomic_down_out_in_history *)
+    (*                   Hrrs Hatm Hrch Hsteps _ H11 H18 H16); clear H16. *)
+
+    (*     eapply MsgOutsRqDownRsUp. *)
+    (*     - pose proof (steps_object_in_system Hsteps _ H19). *)
+    (*       destruct H16 as [pobj [? ?]]; subst. *)
+    (*       eapply Hnodup with (pobj0:= pobj). *)
+    (*       + assumption. *)
+    (*       + reflexivity. *)
+    (*       + eapply rqDown_rsUp_inv_msg. *)
+    (*         rewrite Forall_forall; eassumption. *)
+    (*       + repeat constructor. *)
+    (*         exists (obj_idx obj); right. *)
+    (*         red; auto. *)
+
+    (*     - (* Invariant for each message *) *)
+    (*       apply Forall_app. *)
+    (*       + (* For the others except (rqFrom, rqm) *) *)
+    (*         apply Forall_forall. *)
+    (*         intros [midx msg] ?. *)
+    (*         apply removeOnce_In_NoDup in H16; *)
+    (*           [|apply idsOf_NoDup; assumption]; dest. *)
+
+    (*         pose proof (H3 _ H20). *)
+    (*         destruct H21 as [oidx ?]. *)
+    (*         destruct H21. *)
+    (*         * (* RqDown *) *)
+    (*           exists oidx; left. *)
+    (*           destruct H21. *)
+    (*           split; [assumption|]. *)
+    (*           red in H22. *)
+    (*           red; simpl. *)
+    (*           apply (DisjList_cons_inv eq_nat_dec); [assumption|]. *)
+
+    (*           eapply rqDownMsgOutInv_no_rqDown *)
+    (*             with (oidx := oidx) (rqdm := (midx, msg)) *)
+    (*                  (ooidx := obj_idx obj) (orqdm := (rqFrom, rqm)); *)
+    (*             try eassumption. *)
+    (*           { split; assumption. } *)
+    (*           { split; assumption. } *)
+    (*           { congruence. } *)
+    (*         * (* RsUp *) *)
+    (*           exists oidx; right. *)
+    (*           destruct H21. *)
+    (*           split; [assumption|]. *)
+    (*           red; simpl; intros. *)
+    (*           destruct H23; [subst|auto]. *)
+    (*           red; mred. *)
     
-    Lemma step_msg_outs_ok_RsDownRqDownRule:
-      RsDownRqDownRule dtr sys (obj_idx obj) rule ->
-      MsgOutsCases (orqs +[obj_idx obj <- norq])
-                   (obj_idx obj :: oindsOf hst)
-                   (removeL (id_dec msg_dec) eouts rins ++ routs).
-    Proof.
-      destruct Hrrs as [? [? ?]]; intros.
-      disc_rule_conds.
-      inv_MsgOutsCases.
+    (*       + (* For the new output *) *)
+    (*         repeat constructor. *)
+    (*         exists (obj_idx obj); right. *)
+    (*         split; [red; auto|]. *)
+    (*         red; simpl; intros. *)
+    (*         destruct H16. *)
+    (*         * subst; red; mred. *)
+    (*         * specialize (H14 oidx); destruct H14; exfalso; auto. *)
+    
+    (*     - red; simpl; intros. *)
+    (*       destruct H16; [subst; mred|]. *)
+    (*       red; intros. *)
+    (*       red; simpl. *)
+    (*       apply (DisjList_cons_inv eq_nat_dec); *)
+    (*         [eapply H5; eauto|]. *)
 
-      pose proof (removeL_nil (id_dec msg_dec) [(rsFrom, rsm)]).
-      unfold removeL in H14; unfold Id in *; rewrite H14; clear H14.
-      simpl; disc_rule_conds.
+    (*       intro Hx. *)
+    (*       specialize (H5 _ _ _ H16 H20 H21 _ _ H22 H23 H24). *)
+    (*       red in H5. *)
+    (*       eapply DisjList_In_2 in H19; [|eapply H5]. *)
+    (*       eapply inside_child_outside_parent_case in Hx; *)
+    (*         try eassumption; try apply Hrrs; subst. *)
 
-      eapply MsgOutsRqDownRsUp.
-      - apply HmoutsV.
-      - apply Forall_forall.
-        intros [rqTo rqm] ?.
-        assert (In rqTo (idsOf routs))
-          by (apply in_map_iff; exists (rqTo, rqm); auto).
-        eapply RqRsDownMatch_rq_rs in H11; [|eassumption].
-        destruct H11 as [cidx [rsUp ?]]; dest.
-        rewrite Forall_forall in H15.
-        pose proof (H15 _ H14); simpl in H24.
-        disc_rule_conds.
-        exists cidx; left.
-        split; [red; auto|].
-        red in H13; red; simpl.
-        apply (DisjList_cons_inv eq_nat_dec).
-        + apply DisjList_comm in H13.
-          eapply DisjList_comm, DisjList_SubList;
-            [|eassumption].
-          eapply subtreeIndsOf_child_SubList;
-            [apply Hrrs|assumption].
-        + apply parent_not_in_subtree; [apply Hrrs|auto].
+    (*       pose proof (steps_object_in_system Hsteps _ H16). *)
+    (*       destruct H25 as [dobj [? ?]]; subst. *)
+    (*       good_locking_get dobj; mred. *)
+    (*       red in H26; mred. *)
 
-      - red; simpl; intros.
-        destruct (eq_nat_dec (obj_idx obj) oidx).
-        + subst; clear H14.
-          disc_rule_conds.
-          red; intros.
-          red in H13; red; simpl.
-          apply (DisjList_cons_inv eq_nat_dec).
-          * apply DisjList_comm in H13.
-            eapply DisjList_comm, DisjList_SubList; [|eassumption].
-            apply subtreeIndsOf_child_SubList; [apply Hrrs|assumption].
-          * apply parent_not_in_subtree; [apply Hrrs|assumption].
-        + destruct H14; [exfalso; auto|].
-          disc_rule_conds.
-          exfalso.
-          specialize (H12 _ H14).
-          red in H12; mred.
+    (*       disc_rule_conds. *)
+    (*       specialize (H26 _ H18). *)
+    (*       destruct H26 as [down [rsUp ?]]; dest. *)
+    (*       disc_rule_conds. *)
+    (*       destruct (in_dec eq_nat_dec rsUp _); [auto|]. *)
+    (*       red in H26; dest. *)
+    (*       eapply rqsQ_length_zero_False; eauto. *)
+    
+    (*     - red; simpl; intros. *)
+    (*       destruct H16; [subst; mred|]. *)
+    (*       pose proof (H8 _ _ _ _ _ H16 H20 H21 H22 H23 H24); dest. *)
+    (*       repeat ssplit; [assumption| |]. *)
+    (*       + red in H27. *)
+    (*         red; simpl. *)
+    (*         apply (DisjList_cons_inv eq_nat_dec); [auto|]. *)
+    (*         intro Hx. *)
+    (*         eapply DisjList_In_2 in H19; [|eassumption]. *)
+    (*         eapply inside_child_outside_parent_case in Hx; *)
+    (*           try eassumption; try apply Hrrs; subst. *)
+    (*         disc_rule_conds. *)
 
-      - red; simpl; intros.
-        destruct (eq_nat_dec (obj_idx obj) roidx).
-        + subst; clear H14.
-          disc_rule_conds.
-          repeat split.
-          * intro Hx.
-            eapply RqRsDownMatch_rs_rq in H11; [|eassumption].
-            destruct H11 as [cidx [down ?]]; dest.
-            disc_rule_conds; auto.
-          * red; simpl.
-            apply (DisjList_cons_inv eq_nat_dec).
-            { apply DisjList_comm in H13.
-              eapply DisjList_comm, DisjList_SubList; [|eassumption].
-              apply subtreeIndsOf_child_SubList; [apply Hrrs|assumption].
-            }
-            { apply parent_not_in_subtree; [apply Hrrs|assumption]. }
-          * red; simpl; intros.
-            destruct (eq_nat_dec (obj_idx obj) sidx).
-            { subst; clear H14.
-              disc_rule_conds.
-              apply edgeDownTo_subtreeIndsOf_self_in; [apply Hrrs|congruence].
-            }
-            { destruct H14; [exfalso; auto|].
-              disc_rule_conds.
-              exfalso.
-              specialize (H12 _ H14).
-              red in H12; mred.
-            }
-        + destruct H14; [exfalso; auto|].
-          disc_rule_conds.
-          exfalso.
-          specialize (H12 _ H14).
-          red in H12; mred.
-        
-      - red; repeat (simpl; mred).
-        unfold DownLockNorm; repeat (simpl; mred).
-        rewrite downLocksNorm_orqs_add.
-        + rewrite downLocksNorm_NoDownLocks_zero by assumption.
-          red in H11; dest.
-          rewrite <-H14.
-          assert (length (idsOf routs) > 0).
-          { destruct (idsOf routs); [exfalso; auto|simpl; omega]. }
-          omega.
-        + specialize (H13 (obj_idx obj)).
-          destruct H13; [assumption|].
-          elim H13; apply edgeDownTo_subtreeIndsOf_self_in; [apply Hrrs|congruence].
-    Qed.
+    (*         pose proof (steps_object_in_system Hsteps _ H16). *)
+    (*         destruct H22 as [robj [? ?]]; subst. *)
+    (*         good_locking_get robj; mred. *)
+    (*         red in H23; mred. *)
+    (*         specialize (H23 _ H18). *)
+    (*         destruct H23 as [down [rsUp' ?]]; dest. *)
+    (*         disc_rule_conds. *)
+    (*         destruct (in_dec eq_nat_dec rsUp' _); [auto|]. *)
+    (*         red in H28; dest. *)
+    (*         eapply rqsQ_length_zero_False; eauto. *)
+    (*       + red; simpl; intros. *)
+    (*         destruct H28; [subst|eauto]. *)
+    (*         mred. *)
+
+    (*     - red; repeat (simpl; mred). *)
+    (*       rewrite idsOf_app; simpl. *)
+    (*       rewrite app_length; simpl. *)
+    (*       unfold idsOf; rewrite map_length. *)
+    (*       pose proof (removeOnce_length (id_dec msg_dec) _ _ Hosub); dest. *)
+    (*       unfold Id in *; rewrite H20. *)
+    (*       unfold DownLockNorm; repeat (simpl; mred). *)
+    (*       red in H10. *)
+    (*       unfold idsOf in H10; rewrite map_length in H10. *)
+    (*       omega. *)
+    (*   Qed. *)
+
+    (*   Lemma step_msg_outs_ok_RqFwdRule: *)
+    (*     RqFwdRule dtr sys (obj_idx obj) rule -> *)
+    (*     MsgOutsCases (orqs +[obj_idx obj <- norq]) *)
+    (*                  (obj_idx obj :: oindsOf hst) *)
+    (*                  (removeL (id_dec msg_dec) eouts rins ++ routs). *)
+    (*   Proof. *)
+    (*     destruct Hrrs as [? [? ?]]; intros. *)
+    (*     disc_rule_conds. *)
+    (*     { elim (H19 (obj_idx obj)); do 2 eexists; eauto. } *)
+    (*     { elim (H17 (obj_idx obj)); do 2 eexists; eauto. } *)
+
+    (*     inv_MsgOutsCases. *)
+    (*     pose proof (edgeDownTo_Some H _ H2). *)
+    (*     destruct H19 as [rqUp [rsUp [pidx ?]]]; dest. *)
+    (*     disc_rule_conds. *)
+    (*     assert (In rqFrom (idsOf eouts)) *)
+    (*       by (apply in_map_iff; exists (rqFrom, rqi_msg rqi); auto). *)
+    (*     pose proof (atomic_down_out_in_history *)
+    (*                   Hrrs Hatm Hrch Hsteps _ H2 H22 H21); clear H21. *)
+
+    (*     eapply MsgOutsRqDownRsUp. *)
+    (*     - pose proof (steps_object_in_system Hsteps _ H23). *)
+    (*       destruct H21 as [pobj [? ?]]; subst. *)
+    (*       eapply Hnodup with (pobj0:= pobj). *)
+    (*       + assumption. *)
+    (*       + reflexivity. *)
+    (*       + eapply rqDown_rsUp_inv_msg. *)
+    (*         rewrite Forall_forall; eassumption. *)
+    (*       + apply Forall_forall. *)
+    (*         intros [rqDown rqm] ?. *)
+    (*         rewrite Forall_forall in H20; specialize (H20 _ H24). *)
+    (*         apply in_map with (f:= idOf) in H24; simpl in H24. *)
+    (*         eapply RqRsDownMatch_rq_rs in H4; [|eassumption]. *)
+    (*         destruct H4 as [cidx [rsUp ?]]; dest. *)
+    (*         exists cidx; left. *)
+    (*         red; auto. *)
+
+    (*     - apply Forall_app. *)
+    (*       + apply Forall_forall. *)
+    (*         intros [midx msg] ?. *)
+    (*         apply removeOnce_In_NoDup in H21; *)
+    (*           [|apply idsOf_NoDup; assumption]; dest. *)
+
+    (*         pose proof (H7 _ H24). *)
+    (*         destruct H25 as [oidx ?]. *)
+    (*         destruct H25. *)
+    (*         * (* RqDown *) *)
+    (*           exists oidx; left. *)
+    (*           destruct H25. *)
+    (*           split; [assumption|]. *)
+    (*           red in H26. *)
+    (*           red; simpl. *)
+    (*           apply (DisjList_cons_inv eq_nat_dec); [assumption|]. *)
+
+    (*           eapply rqDownMsgOutInv_no_rqDown *)
+    (*             with (oidx := oidx) (rqdm := (midx, msg)) *)
+    (*                  (ooidx := obj_idx obj) (orqdm := (rqFrom, rqi_msg rqi)); *)
+    (*             try eassumption. *)
+    (*           { split; assumption. } *)
+    (*           { split; assumption. } *)
+    (*           { congruence. } *)
+    (*         * (* RsUp *) *)
+    (*           exists oidx; right. *)
+    (*           destruct H25. *)
+    (*           split; [assumption|]. *)
+
+    (*           red; simpl; intros. *)
+    (*           destruct (eq_nat_dec (obj_idx obj) oidx0). *)
+    (*           { subst; exfalso. *)
+    (*             eapply rsUpMsgOutInv_no_rqDown *)
+    (*               with (oidx := oidx) (rsum := (midx, msg)) *)
+    (*                    (ooidx := obj_idx obj) (orqdm := (rqFrom, rqi_msg rqi)); *)
+    (*               try eassumption. *)
+    (*             { split; assumption. } *)
+    (*             { split; assumption. } *)
+    (*           } *)
+    (*           { destruct H27; [exfalso; auto|]. *)
+    (*             specialize (H26 _ H27 H28). *)
+    (*             red; mred. *)
+    (*           } *)
+
+    (*       + apply Forall_forall. *)
+    (*         intros [rqTo rqm] ?. *)
+    (*         assert (In rqTo (idsOf routs)) *)
+    (*           by (apply in_map_iff; exists (rqTo, rqm); auto). *)
+    (*         eapply RqRsDownMatch_rq_rs in H4; [|eassumption]. *)
+    (*         destruct H4 as [cidx [rsUp ?]]; dest. *)
+    (*         rewrite Forall_forall in H20. *)
+    (*         pose proof (H20 _ H21); simpl in H29. *)
+    (*         exists cidx; left. *)
+    (*         split; [red; auto|]. *)
+    (*         red in H18; red; simpl. *)
+    (*         apply (DisjList_cons_inv eq_nat_dec). *)
+    (*         { apply DisjList_comm in H18. *)
+    (*           eapply DisjList_comm, DisjList_SubList; *)
+    (*             [|eassumption]. *)
+    (*           eapply subtreeIndsOf_child_SubList; *)
+    (*             [apply Hrrs|assumption]. *)
+    (*         } *)
+    (*         { apply parent_not_in_subtree; [apply Hrrs|auto]. } *)
+
+    (*     - red; simpl; intros. *)
+    (*       destruct (eq_nat_dec (obj_idx obj) oidx). *)
+    (*       + subst; mred. *)
+    (*         red; intros. *)
+    (*         red in H18; red; simpl. *)
+    (*         apply (DisjList_cons_inv eq_nat_dec). *)
+    (*         * eapply DisjList_comm in H18. *)
+    (*           eapply DisjList_comm, DisjList_SubList; [|eassumption]. *)
+    (*           apply subtreeIndsOf_child_SubList; *)
+    (*             [apply Hrrs|assumption]. *)
+    (*         * eapply parent_not_in_subtree; [apply Hrrs|auto]. *)
+    (*       + destruct H21; [exfalso; auto|]. *)
+    (*         mred; specialize (H11 _ _ _ H21 H24 H25). *)
+    (*         red; intros. *)
+    (*         specialize (H11 _ _ H26 H27 H28). *)
+    (*         red in H11. *)
+    (*         red; simpl; intros. *)
+    (*         apply (DisjList_cons_inv eq_nat_dec); [assumption|]. *)
+    (*         eapply DisjList_In_2 in H23; [|eapply H11]. *)
+    (*         eapply outside_child_in in H23; try apply Hrrs; [|eassumption]. *)
+    (*         destruct H23; [subst; exfalso|assumption]. *)
+    (*         pose proof (steps_object_in_system Hsteps _ H21). *)
+    (*         destruct H23 as [oobj [? ?]]; subst. *)
+    (*         good_locking_get oobj. *)
+    (*         red in H29; mred. *)
+
+    (*         disc_rule_conds. *)
+    (*         specialize (H29 _ H22). *)
+    (*         destruct H29 as [down [rsUp ?]]; dest. *)
+    (*         disc_rule_conds. *)
+    (*         destruct (in_dec eq_nat_dec (rqi_midx_rsb rqi) _); [auto|]. *)
+    (*         red in H29; dest. *)
+    (*         eapply rqsQ_length_zero_False; eauto. *)
+    
+    (*     - red; simpl; intros. *)
+    (*       destruct (eq_nat_dec (obj_idx obj) roidx); *)
+    (*         [subst; exfalso; mred; solve_midx_false|]. *)
+    (*       destruct H21; [exfalso; auto|]. *)
+    (*       mred. *)
+    (*       specialize (H13 _ _ _ _ _ H21 H24 H25 H26 H27 H28); dest. *)
+    (*       repeat ssplit; [assumption| |]. *)
+    (*       + red in H29. *)
+    (*         red; simpl. *)
+    (*         apply (DisjList_cons_inv eq_nat_dec); [auto|]. *)
+    (*         intro Hx. *)
+    (*         eapply DisjList_In_2 in H23; [|apply H29]. *)
+    (*         eapply inside_child_outside_parent_case in Hx; *)
+    (*           try eassumption; try apply Hrrs; subst. *)
+    (*         disc_rule_conds. *)
+
+    (*         pose proof (steps_object_in_system Hsteps _ H21). *)
+    (*         destruct H26 as [robj [? ?]]; subst. *)
+    (*         good_locking_get robj; mred. *)
+    (*         red in H27; mred. *)
+    (*         specialize (H27 _ H22). *)
+    (*         destruct H27 as [down [rsUp ?]]; dest. *)
+    (*         disc_rule_conds. *)
+    (*         destruct (in_dec eq_nat_dec (rqi_midx_rsb rqi) _); [auto|]. *)
+    (*         red in H31; dest. *)
+    (*         eapply rqsQ_length_zero_False; eauto. *)
+    (*       + red; simpl; intros. *)
+    (*         destruct (eq_nat_dec (obj_idx obj) sidx). *)
+    (*         * subst; clear H31; mred. *)
+    (*           pose proof (steps_object_in_system Hsteps _ H23). *)
+    (*           destruct H31 as [pobj [? ?]]; subst. *)
+    (*           good_locking_get pobj. *)
+    (*           eapply downLockInvORq_down_rqsQ_length_one_locked in H32; *)
+    (*             try eassumption; *)
+    (*             [|eapply rqsQ_length_ge_one; *)
+    (*               [eassumption|apply FirstMP_InMP; assumption]]. *)
+    (*           destruct H32 as [prqid ?]; dest. *)
+    (*           remember (orqs@[obj_idx pobj]) as pporq; apply eq_sym in Heqpporq. *)
+    (*           destruct pporq as [pporq|]; [simpl in H32|discriminate]. *)
+    (*           eapply inside_child_in; [apply Hrrs|eassumption|]. *)
+    (*           eapply H30; eassumption. *)
+    (*         * destruct H31; [exfalso; auto|]. *)
+    (*           mred; eauto. *)
+    
+    (*     - red; repeat (simpl; mred). *)
+    (*       rewrite idsOf_app; simpl. *)
+    (*       rewrite app_length; simpl. *)
+    (*       unfold idsOf; rewrite map_length. *)
+    (*       pose proof (removeOnce_length (id_dec msg_dec) _ _ Hosub); dest. *)
+    (*       unfold Id in *; rewrite H24. *)
+    (*       unfold DownLockNorm; repeat (simpl; mred). *)
+
+    (*       red in H4; dest; rewrite <-H25. *)
+    (*       rewrite downLocksNorm_orqs_add. *)
+    (*       + assert (length (idsOf routs) > 0) *)
+    (*           by (destruct (idsOf routs); [exfalso; auto|simpl; omega]). *)
+    (*         red in H15. *)
+    (*         unfold idsOf in H15; rewrite map_length in H15. *)
+    (*         rewrite H15. *)
+    (*         unfold idsOf in *. *)
+    (*         omega. *)
+    (*       + specialize (H7 _ Hosub). *)
+    (*         destruct H7 as [oidx ?]. *)
+    (*         destruct H7; [|destruct H7; disc_rule_conds]. *)
+    (*         destruct H7; disc_rule_conds. *)
+    (*         red in H18. *)
+    (*         eapply DisjList_In_1. *)
+    (*         * eassumption. *)
+    (*         * apply rsEdgeUpFrom_subtreeIndsOf_self_in; [apply Hrrs|congruence]. *)
+    (*   Qed. *)
+
+    (*   Lemma step_msg_outs_ok_RsBackRule: *)
+    (*     RsBackRule rule -> *)
+    (*     MsgOutsCases (orqs +[obj_idx obj <- norq]) *)
+    (*                  (obj_idx obj :: oindsOf hst) *)
+    (*                  (removeL (id_dec msg_dec) eouts rins ++ routs). *)
+    (*   Proof. *)
+    (*     destruct Hrrs as [? [? ?]]; intros. *)
+    (*     good_footprint_get (obj_idx obj). *)
+    (*     disc_rule_conds. *)
+    (*     - (** [RsDownDown] *) *)
+    (*       inv_MsgOutsCases. *)
+    (*       disc_rule_conds. *)
+    (*       destruct (id_dec msg_dec i i) as [_|]; [simpl|exfalso; auto]. *)
+
+    (*       eapply MsgOutsRsDown. *)
+    (*       + split; [red; simpl; eauto|]. *)
+    (*         red; simpl. *)
+    (*         apply (DisjList_cons_inv eq_nat_dec). *)
+    (*         * red in H16; apply DisjList_comm in H16. *)
+    (*           eapply DisjList_comm, DisjList_SubList; [|eassumption]. *)
+    (*           apply subtreeIndsOf_child_SubList; [apply Hrrs|assumption]. *)
+    (*         * apply parent_not_in_subtree; [apply Hrrs|assumption]. *)
+    (*       + red; simpl; intros. *)
+    (*         destruct H18; subst. *)
+    (*         * red; repeat (simpl; mred). *)
+    (*         * specialize (H15 _ H18). *)
+    (*           red in H15; red. *)
+    (*           repeat (simpl; mred). *)
+
+    (*     - (** [RsUpDown] *) *)
+    (*       inv_MsgOutsCases. *)
+    (*       + exfalso. *)
+    (*         eapply SubList_singleton_NoDup in Hosub; *)
+    (*           [|apply idsOf_NoDup, HminsV]. *)
+    (*         destruct Hosub; [exfalso; auto|subst]. *)
+    (*         rewrite <-H17 in H10. *)
+    (*         eapply RqRsDownMatch_rs_rq in H10; [|left; reflexivity]. *)
+    (*         destruct H10 as [cidx [down ?]]; dest. *)
+    (*         disc_rule_conds. *)
+    (*         solve_midx_false. *)
+
+    (*       + pose proof (edgeDownTo_Some H _ H9). *)
+    (*         destruct H18 as [rqUp [rsUp [pidx ?]]]; dest. *)
+    (*         disc_rule_conds. *)
+    (*         rewrite Forall_forall in H11. *)
+
+    (*         (* Different proofs whether the object is part of the history or not *) *)
+    (*         destruct (in_dec eq_nat_dec (obj_idx obj) (oindsOf hst)). *)
+    (*         * (* If the object is in the history, we can use 1) [DownLockRootInv] *)
+     (*            * to say all downlocks are in the tree of the object and 2) the RsUp *)
+     (*            * invariants to say there are no downlocks in the tree. *)
+     (*            *) *)
+    (*           specialize (H15 _ _ _ _ _ i Hporq H14 H5 H9 H19); dest. *)
+    (*           specialize (H13 _ _ _ i Hporq H14). *)
+    (*           assert (removeL (id_dec msg_dec) eouts rins = nil). *)
+    (*           { eapply SubList_NoDup_length_eq_removeL_nil. *)
+    (*             { assumption. } *)
+    (*             { apply idsOf_NoDup, HminsV. } *)
+    (*             { (* [length rins = length eouts] *) *)
+    (*               (** FIXME: must use [downLocksNorm_rsUps] here, but it requires *)
+     (*                * strengthening the invariant about the RsDown-root to appear *)
+     (*                * at most once in the history. *)
+     (*                *) *)
+    (*               admit. *)
+    (*             } *)
+    (*           } *)
+    (*           rewrite H21; simpl; clear H21. *)
+    
+    (*           eapply MsgOutsRsDown. *)
+    (*           { split; [red; eauto|]. *)
+    (*             red; simpl. *)
+    (*             apply (DisjList_cons_inv eq_nat_dec); [assumption|]. *)
+    (*             apply parent_not_in_subtree; [apply Hrrs|assumption]. *)
+    (*           } *)
+    (*           { simpl; red; simpl; intros. *)
+    (*             destruct (eq_nat_dec (obj_idx obj) oidx); *)
+    (*               [subst; red; repeat (simpl; mred)|]. *)
+    (*             destruct H21; [exfalso; auto|]. *)
+    (*             eapply downLockCoverInv_DownLockInRoot_NoDownLock with (ridx:= obj_idx obj). *)
+    (*             { auto. } *)
+    (*             { eassumption. } *)
+    (*             { apply eq_sym; eassumption. } *)
+    (*             { intros [rrsUp rrsm] ?. *)
+    (*               rewrite <-H17 in H10. *)
+    (*               assert (In rrsUp (idsOf rins)) *)
+    (*                 by (apply in_map with (f:= idOf) in H22; assumption). *)
+    (*               eapply RqRsDownMatch_rs_rq in H10; [|eassumption]; clear H23. *)
+    (*               destruct H10 as [rcidx [rdown ?]]; dest. *)
+    (*               apply Hosub in H22. *)
+    (*               specialize (H11 _ H22). *)
+    (*               destruct H11 as [cidx ?]. *)
+    (*               destruct H11; [destruct H11; disc_rule_conds; solve_midx_false|]. *)
+    (*               exists cidx. *)
+    (*               apply rsUpMsgOutInv_orqs_downRq_remove; assumption. *)
+    (*             } *)
+    (*             { assumption. } *)
+    (*             { apply downLockInRoot_orqs_downRq_remove; assumption. } *)
+    (*           } *)
+
+    (*         * (* When [~ In (obj_idx obj) (oindsOf hst)] *) *)
+    (*           admit. *)
+
+    (*     - (** [RsUpUp] *) *)
+    (*       inv_MsgOutsCases. *)
+    (*       { exfalso. *)
+    (*         eapply SubList_singleton_NoDup in Hosub; *)
+    (*           [|apply idsOf_NoDup, HminsV]. *)
+    (*         destruct Hosub; [exfalso; auto|subst]. *)
+    (*         rewrite <-H17 in H5. *)
+    (*         eapply RqRsDownMatch_rs_rq in H5; [|left; reflexivity]. *)
+    (*         destruct H5 as [cidx [down ?]]; dest. *)
+    (*         disc_rule_conds. *)
+    (*         solve_midx_false. *)
+    (*       } *)
+
+    (*       pose proof (edgeDownTo_Some H _ H2). *)
+    (*       destruct H15 as [rqUp [rsUp [pidx ?]]]; dest. *)
+    (*       rewrite Forall_forall in H9. *)
+    (*       disc_rule_conds. *)
+
+    (*       (* Different proofs whether the object is part of the history or not *) *)
+    (*       destruct (in_dec eq_nat_dec (obj_idx obj) (oindsOf hst)). *)
+    (*       + (* Need to have just one child of the incoming RsUp messages. *) *)
+    (*         assert (exists rsFrom rsfm, In (rsFrom, rsfm) rins). *)
+    (*         { destruct rins as [|[rsFrom rsfm] ?]; [exfalso; auto|]. *)
+    (*           do 2 eexists; left; reflexivity. *)
+    (*         } *)
+    (*         destruct H16 as [rsFrom [rsfm ?]]. *)
+    (*         rewrite Forall_forall in H8. *)
+    (*         specialize (H8 _ H16); simpl in H8. *)
+    (*         assert (In rsFrom (idsOf rins)) *)
+    (*           by (apply in_map with (f:= idOf) in H16; assumption). *)
+    (*         rewrite <-H17 in H5. *)
+    (*         eapply RqRsDownMatch_rs_rq in H5; [|eassumption]; clear H19. *)
+    (*         destruct H5 as [ccidx [down ?]]; dest. *)
+    (*         eapply Hosub in H16. *)
+    (*         assert (In rsFrom (idsOf eouts)) *)
+    (*           by (apply in_map with (f:= idOf) in H16; assumption). *)
+    (*         pose proof (atomic_rsUp_out_in_history *)
+    (*                       Hrrs Hatm Hrch Hsteps _ H21 H23); clear H23. *)
+
+    (*         eapply MsgOutsRqDownRsUp. *)
+    (*         * (* [NoDup] for [RsUpUp] *) *)
+    (*           eapply Hnodup. *)
+    (*           { admit. } *)
+    (*           { admit. } *)
+    (*           { eapply rqDown_rsUp_inv_msg. *)
+    (*             rewrite Forall_forall; eassumption. *)
+    (*           } *)
+    (*           { repeat constructor. *)
+    (*             exists (obj_idx obj); right. *)
+    (*             red; auto. *)
+    (*           } *)
+
+    (*         * apply Forall_app. *)
+    (*           { apply Forall_forall. *)
+    (*             intros [midx msg] ?. *)
+    (*             apply removeL_In_NoDup in H23; [|apply idsOf_NoDup; assumption]; dest. *)
+    (*             pose proof (H9 _ H25). *)
+    (*             destruct H26 as [oidx ?]; destruct H26. *)
+    (*             { exists oidx; left. *)
+    (*               destruct H26. *)
+    (*               split; [assumption|]. *)
+    (*               red; simpl. *)
+    (*               apply (DisjList_cons_inv eq_nat_dec); [auto|]. *)
+    (*               eapply rqDownMsgOutInv_no_rsUp with (orsum := (rsFrom, rsfm)); *)
+    (*                 try eassumption. *)
+    (*               { split; assumption. } *)
+    (*               { reflexivity. } *)
+    (*               { red; auto. } *)
+    (*             } *)
+    (*             { exists oidx; right. *)
+    (*               destruct H26. *)
+    (*               split; [assumption|]. *)
+    (*               red; simpl; intros. *)
+    (*               destruct (eq_nat_dec (obj_idx obj) oidx0); *)
+    (*                 [subst; red; repeat (simpl; mred)|]. *)
+    (*               destruct H28; [exfalso; auto|]. *)
+    (*               red; mred. *)
+    (*               eapply H27; eauto. *)
+    (*             } *)
+    (*           } *)
+    (*           { repeat constructor. *)
+    (*             exists (obj_idx obj); right. *)
+    (*             split; [red; auto|]. *)
+    (*             red; simpl; intros. *)
+    (*             destruct (eq_nat_dec (obj_idx obj) oidx); *)
+    (*               [subst; red; repeat (simpl; mred)|]. *)
+    (*             destruct H23; [exfalso; auto|]. *)
+    (*             red; mred. *)
+    (*             apply subtreeIndsOf_composed in H25; [|apply Hrrs]. *)
+    (*             destruct H25; [exfalso; auto|]. *)
+    (*             destruct H25 as [cidx [? ?]]. *)
+    (*             pose proof (parentIdxOf_Some H _ H25). *)
+    (*             destruct H27 as [crqUp [crsUp [cdown ?]]]; dest. *)
+    (*             destruct (in_dec eq_nat_dec crsUp rqi.(rqi_minds_rss)). *)
+    (*             { rewrite <-H17 in i0. *)
+    (*               apply in_map_iff in i0. *)
+    (*               destruct i0 as [[crsUp' crsm] [? ?]]; simpl in *; subst. *)
+    (*               apply Hosub in H31. *)
+    (*               specialize (H9 _ H31). *)
+    (*               destruct H9 as [rcidx ?]. *)
+    (*               destruct H9; [destruct H9; disc_rule_conds; solve_midx_false|]. *)
+    (*               destruct H9; disc_rule_conds. *)
+    (*               specialize (H30 _ H23 H26). *)
+    (*               red in H30; destruct (orqs@[oidx]); auto. *)
+    (*             } *)
+    (*             { specialize (H10 _ _ _ i Hporq H14). *)
+    (*               red in H10. *)
+    (*               specialize (H10 _ _ H25 H28 n0 oidx). *)
+    (*               exfalso; destruct H10; eauto. *)
+    (*             } *)
+    (*           } *)
+
+    (*         * red; simpl; intros. *)
+    (*           destruct (eq_nat_dec (obj_idx obj) oidx); *)
+    (*             [subst; red; repeat (simpl; mred)|]. *)
+    (*           destruct H23; [exfalso; auto|]. *)
+    (*           mred; red; intros. *)
+    (*           red; simpl; intros. *)
+    (*           apply (DisjList_cons_inv eq_nat_dec); [eapply H10; eauto|]. *)
+    (*           specialize (H10 _ _ _ H23 H25 H26). *)
+    (*           specialize (H10 _ _ H27 H28 H29). *)
+    (*           eapply outside_parent_out; [apply Hrrs| |eassumption]. *)
+    (*           eapply DisjList_In_2; eassumption. *)
+
+    (*         * red; simpl; intros. *)
+    (*           destruct (eq_nat_dec (obj_idx obj) roidx); [subst; mred|]. *)
+    (*           destruct H23; [exfalso; auto|]. *)
+    (*           mred. *)
+    (*           specialize (H11 _ _ _ _ _ H23 H25 H26 H27 H28 H29); dest. *)
+    (*           repeat split; [assumption| |]. *)
+    (*           { red; simpl. *)
+    (*             apply (DisjList_cons_inv eq_nat_dec); [auto|]. *)
+    (*             eapply outside_parent_out; [apply Hrrs| |eassumption]. *)
+    (*             eapply DisjList_In_2; eassumption. *)
+    (*           } *)
+    (*           { red; simpl; intros. *)
+    (*             destruct (eq_nat_dec (obj_idx obj) sidx); [subst; mred|]. *)
+    (*             destruct H32; [exfalso; auto|]. *)
+    (*             mred; eauto. *)
+    (*           } *)
+
+    (*         * red; repeat (simpl; mred). *)
+    (*           rewrite idsOf_app, app_length; simpl. *)
+    (*           unfold DownLockNorm; repeat (simpl; mred). *)
+    (*           (* [MsgOutsNormInv] for [RsUpUp] *) *)
+    (*           admit. *)
+
+    (*       + (* When [~ In (obj_idx obj) (oindsOf hst)] *) *)
+    (*         admit. *)
+    
+    (*   Admitted. *)
+    
+    (*   Lemma step_msg_outs_ok_RsDownRqDownRule: *)
+    (*     RsDownRqDownRule dtr sys (obj_idx obj) rule -> *)
+    (*     MsgOutsCases (orqs +[obj_idx obj <- norq]) *)
+    (*                  (obj_idx obj :: oindsOf hst) *)
+    (*                  (removeL (id_dec msg_dec) eouts rins ++ routs). *)
+    (*   Proof. *)
+    (*     destruct Hrrs as [? [? ?]]; intros. *)
+    (*     disc_rule_conds. *)
+    (*     inv_MsgOutsCases. *)
+
+    (*     pose proof (removeL_nil (id_dec msg_dec) [(rsFrom, rsm)]). *)
+    (*     unfold removeL in H14; unfold Id in *; rewrite H14; clear H14. *)
+    (*     simpl; disc_rule_conds. *)
+
+    (*     eapply MsgOutsRqDownRsUp. *)
+    (*     - apply HmoutsV. *)
+    (*     - apply Forall_forall. *)
+    (*       intros [rqTo rqm] ?. *)
+    (*       assert (In rqTo (idsOf routs)) *)
+    (*         by (apply in_map_iff; exists (rqTo, rqm); auto). *)
+    (*       eapply RqRsDownMatch_rq_rs in H11; [|eassumption]. *)
+    (*       destruct H11 as [cidx [rsUp ?]]; dest. *)
+    (*       rewrite Forall_forall in H15. *)
+    (*       pose proof (H15 _ H14); simpl in H24. *)
+    (*       disc_rule_conds. *)
+    (*       exists cidx; left. *)
+    (*       split; [red; auto|]. *)
+    (*       red in H13; red; simpl. *)
+    (*       apply (DisjList_cons_inv eq_nat_dec). *)
+    (*       + apply DisjList_comm in H13. *)
+    (*         eapply DisjList_comm, DisjList_SubList; *)
+    (*           [|eassumption]. *)
+    (*         eapply subtreeIndsOf_child_SubList; *)
+    (*           [apply Hrrs|assumption]. *)
+    (*       + apply parent_not_in_subtree; [apply Hrrs|auto]. *)
+
+    (*     - red; simpl; intros. *)
+    (*       destruct (eq_nat_dec (obj_idx obj) oidx). *)
+    (*       + subst; clear H14. *)
+    (*         disc_rule_conds. *)
+    (*         red; intros. *)
+    (*         red in H13; red; simpl. *)
+    (*         apply (DisjList_cons_inv eq_nat_dec). *)
+    (*         * apply DisjList_comm in H13. *)
+    (*           eapply DisjList_comm, DisjList_SubList; [|eassumption]. *)
+    (*           apply subtreeIndsOf_child_SubList; [apply Hrrs|assumption]. *)
+    (*         * apply parent_not_in_subtree; [apply Hrrs|assumption]. *)
+    (*       + destruct H14; [exfalso; auto|]. *)
+    (*         disc_rule_conds. *)
+    (*         exfalso. *)
+    (*         specialize (H12 _ H14). *)
+    (*         red in H12; mred. *)
+
+    (*     - red; simpl; intros. *)
+    (*       destruct (eq_nat_dec (obj_idx obj) roidx). *)
+    (*       + subst; clear H14. *)
+    (*         disc_rule_conds. *)
+    (*         repeat split. *)
+    (*         * intro Hx. *)
+    (*           eapply RqRsDownMatch_rs_rq in H11; [|eassumption]. *)
+    (*           destruct H11 as [cidx [down ?]]; dest. *)
+    (*           disc_rule_conds; auto. *)
+    (*         * red; simpl. *)
+    (*           apply (DisjList_cons_inv eq_nat_dec). *)
+    (*           { apply DisjList_comm in H13. *)
+    (*             eapply DisjList_comm, DisjList_SubList; [|eassumption]. *)
+    (*             apply subtreeIndsOf_child_SubList; [apply Hrrs|assumption]. *)
+    (*           } *)
+    (*           { apply parent_not_in_subtree; [apply Hrrs|assumption]. } *)
+    (*         * red; simpl; intros. *)
+    (*           destruct (eq_nat_dec (obj_idx obj) sidx). *)
+    (*           { subst; clear H14. *)
+    (*             disc_rule_conds. *)
+    (*             apply edgeDownTo_subtreeIndsOf_self_in; [apply Hrrs|congruence]. *)
+    (*           } *)
+    (*           { destruct H14; [exfalso; auto|]. *)
+    (*             disc_rule_conds. *)
+    (*             exfalso. *)
+    (*             specialize (H12 _ H14). *)
+    (*             red in H12; mred. *)
+    (*           } *)
+    (*       + destruct H14; [exfalso; auto|]. *)
+    (*         disc_rule_conds. *)
+    (*         exfalso. *)
+    (*         specialize (H12 _ H14). *)
+    (*         red in H12; mred. *)
+    
+    (*     - red; repeat (simpl; mred). *)
+    (*       unfold DownLockNorm; repeat (simpl; mred). *)
+    (*       rewrite downLocksNorm_orqs_add. *)
+    (*       + rewrite downLocksNorm_NoDownLocks_zero by assumption. *)
+    (*         red in H11; dest. *)
+    (*         rewrite <-H14. *)
+    (*         assert (length (idsOf routs) > 0). *)
+    (*         { destruct (idsOf routs); [exfalso; auto|simpl; omega]. } *)
+    (*         omega. *)
+    (*       + specialize (H13 (obj_idx obj)). *)
+    (*         destruct H13; [assumption|]. *)
+    (*         elim H13; apply edgeDownTo_subtreeIndsOf_self_in; [apply Hrrs|congruence]. *)
+    (*   Qed. *)
 
   End InternalStep.
   
   Lemma atomic_msg_outs_ok:
     forall inits ins hst outs eouts,
       Atomic msg_dec inits ins hst outs eouts ->
-      Forall (NonRqUpL dtr) hst ->
       forall s1 s2,
         Reachable (steps step_m) sys s1 ->
         steps step_m sys s1 hst s2 ->
-        MsgOutsCases s2.(bst_orqs) (oindsOf hst) eouts.
+        MsgOutsCases (oindsOf hst) s1.(bst_orqs) s2.(bst_orqs) eouts.
   Proof.
     destruct Hrrs as [? [? ?]].
     induction 1; simpl; intros; subst;
-      [inv H2; inv_steps; eapply step_msg_outs_ok; eauto|].
+      [inv_steps; eapply step_msg_outs_ok; eauto|].
 
-    inv H8; inv_steps.
-    specialize (IHAtomic H11 _ _ H9 H12); dest.
+    inv_steps.
+    specialize (IHAtomic _ _ H8 H10).
 
     assert (Reachable (steps step_m) sys st2) by eauto.
     pose proof (footprints_ok H0 H5) as Hftinv.
     pose proof (downLockInv_ok H0 H H5) as Hdlinv.
-    pose proof (nonRqUpL_atomic_msg_outs_no_rqUp Hrrs H2 H11 H9 H12).
-    eapply SubList_forall in H6; [|eassumption].
     assert (forall pidx pobj,
                parentIdxOf dtr oidx = Some pidx ->
                In pobj (sys_objs sys) ->
@@ -1783,13 +2014,90 @@ Section MsgOutCases.
     good_rqrs_rule_cases rule; simpl in *.
 
     - eapply step_msg_outs_ok_ImmDownRule; eauto.
-    - eapply step_msg_outs_ok_ImmUpRule; eauto.
-    - eapply step_msg_outs_ok_RqFwdRule; eauto.
-    - eapply step_msg_outs_ok_RsBackRule; eauto.
-    - eapply step_msg_outs_ok_RsDownRqDownRule; eauto.
+    (* - eapply step_msg_outs_ok_ImmUpRule; eauto. *)
+    (* - eapply step_msg_outs_ok_RqFwdRule; eauto. *)
+    (* - eapply step_msg_outs_ok_RsBackRule; eauto. *)
+    (* - eapply step_msg_outs_ok_RsDownRqDownRule; eauto. *)
+  Admitted.
+
+  Corollary atomic_rqDown_covers:
+    forall oidx rqDown,
+      RqDownMsgTo oidx rqDown ->
+      forall inits ins hst outs eouts,
+        In rqDown eouts ->
+        Atomic msg_dec inits ins hst outs eouts ->
+        forall st1 st2,
+          Reachable (steps step_m) sys st1 ->
+          steps step_m sys st1 hst st2 ->
+          DisjList (oindsOf hst) (subtreeIndsOf dtr oidx).
+  Proof.
+    destruct Hrrs as [? [? ?]]; intros.
+    eapply atomic_msg_outs_ok in H4; eauto.
+    inv H4.
+    - exfalso.
+      Common.dest_in.
+      destruct H7.
+      repeat disc_msg_case.
+      solve_midx_false.
+    - exfalso.
+      Common.dest_in.
+      destruct H7.
+      repeat disc_msg_case.
+      rewrite H2 in H3; discriminate.
+    - rewrite Forall_forall in H8.
+      specialize (H8 _ H3).
+      destruct H8 as [doidx ?].
+      destruct H4.
+      + destruct H4.
+        repeat disc_msg_case.
+        disc_rule_conds.
+      + exfalso.
+        destruct H4.
+        repeat disc_msg_case.
+        solve_midx_false.
+  Qed.
+
+  Corollary atomic_rsDown_covers:
+    forall oidx rsDown,
+      RsDownMsgTo oidx rsDown ->
+      forall inits ins hst outs eouts,
+        In rsDown eouts ->
+        Atomic msg_dec inits ins hst outs eouts ->
+        Forall (NonRqUpL dtr) hst ->
+        forall st1 st2,
+          Reachable (steps step_m) sys st1 ->
+          steps step_m sys st1 hst st2 ->
+          DisjList (oindsOf hst) (subtreeIndsOf dtr oidx).
+  Proof.
+    destruct Hrrs as [? [? ?]]; intros.
+    pose proof H4.
+    eapply atomic_msg_outs_ok in H8; eauto.
+    inv H8.
+    - exfalso.
+      Common.dest_in.
+      destruct H9.
+      repeat disc_msg_case.
+      solve_midx_false.
+    - Common.dest_in.
+      destruct H9.
+      repeat disc_msg_case.
+      repeat disc_rule_minds.
+      eapply disjExceptUpLocked_no_UpLockedNew_disj; [eassumption|].
+      eapply atomic_NonRqUp_no_new_uplocks; eauto.
+    - exfalso.
+      rewrite Forall_forall in H10.
+      specialize (H10 _ H3).
+      destruct H10 as [doidx ?].
+      destruct H8.
+      + destruct H8.
+        repeat disc_msg_case.
+        rewrite H2 in H8; discriminate.
+      + destruct H8.
+        repeat disc_msg_case.
+        solve_midx_false.
   Qed.
   
-End MsgOutCases.
+End Coverage.
 
 Close Scope list.
 Close Scope fmap.
